TraceEquality for modules that have been re-merged after a file separation now Qeds.

PProperties.v
@@ -1025,11 +1025,6 @@ Proof.
   - exists o'', nil;
       repeat split; eauto using Permutation_sym; try econstructor; eauto.
     apply Forall2_RegInit_keymatch; assumption.
-  (* - unfold UpdRegs in HPUpdRegs; apply PStep_Step in HPStep; dest. *)
-  (* - specialize (key_perm_eq _ _ (Permutation_sym HUpdRegs1)) as TMP;dest. *)
-  (*   exists x, nil. *)
-  (*   repeat split; eauto using Permutation_sym; econstructor; auto. *)
-  (*   eapply RegInit_generalized_list; eauto. *)
   - specialize (WfNoDups H) as TMP; dest.
     apply PStep_Step in HPStep; dest.
     unfold PUpdRegs in HPUpdRegs; dest.
@@ -1103,5 +1098,1900 @@ Proof.
   - specialize (List_FullLabel_perm_Lists_WeakInclusions H5) as trans.
     apply (WeakInclusionsTrans H3 trans).
 Qed.
-  
 
+Section PSubsteps_rewrite.
+  
+  Lemma PSubsteps_rewrite_regs m o1 o2 l:
+    (o1 [=] o2) ->
+    PSubsteps m o1 l ->
+    PSubsteps m o2 l.
+  Proof.
+    induction 2.
+    - econstructor 1.
+      rewrite <- H; assumption.
+    - econstructor 2;[rewrite <- H|apply HInRules|apply (PSemAction_rewrite_state H) in HPAction; apply HPAction| | |apply HLabel| | | |];assumption.
+    - econstructor 3;[rewrite <- H|apply HInMeths|apply (PSemAction_rewrite_state H) in HPAction; apply HPAction| | |apply HLabel| | |];assumption.
+  Qed.
+
+  Lemma PSubsteps_rewrite_lists m o l1 l2:
+    (l1 [=] l2) ->
+    PSubsteps m o l1 ->
+    PSubsteps m o l2.
+  Proof.
+    induction 2.
+    - apply Permutation_nil in H; rewrite H.
+      econstructor 1; assumption.
+    - econstructor 2; eauto.
+      rewrite H in HLabel.
+      assumption.
+    - econstructor 3; eauto.
+      rewrite H in HLabel.
+      assumption.
+  Qed.
+
+  Lemma PSubsteps_rewrite_both m o1 o2 l1 l2 :
+    o1 [=] o2 ->
+    l1 [=] l2 ->
+    PSubsteps m o1 l1 ->
+    PSubsteps m o2 l2.
+  Proof.
+    intros; apply (PSubsteps_rewrite_regs H) in H1; apply (PSubsteps_rewrite_lists H0) in H1; assumption.
+  Qed.
+
+  Inductive BaseModule_perm : BaseModule -> BaseModule -> Prop :=
+  | perm_equiv m m' (HRegsPerm : getRegisters m [=] getRegisters m')
+               (HMethsPerm : getMethods m [=] getMethods m')
+               (HRulesPerm : getRules m [=] getRules m') :
+      BaseModule_perm m m'.
+  
+  Lemma BaseModule_perm_refl m :
+    BaseModule_perm m m.
+  Proof.
+    constructor; auto.
+  Qed.
+
+  Lemma BaseModule_perm_sym m m' :
+    BaseModule_perm m m' -> BaseModule_perm m' m.
+  Proof.
+    intro; induction H; constructor; eauto using Permutation_sym.
+  Qed.
+
+  Lemma BaseModule_perm_trans m m' m'':
+    BaseModule_perm m m' -> BaseModule_perm m' m'' -> BaseModule_perm m m''.
+  Proof.
+    intros.
+    induction H, H0; constructor; eauto using Permutation_trans.
+  Qed.
+
+  Global Instance BaseModule_perm_Equivalence : Equivalence (@BaseModule_perm) | 10 := {
+    Equivalence_Reflexive := @BaseModule_perm_refl;
+    Equivalence_Symmetric := @BaseModule_perm_sym;
+    Equivalence_Transitive:= @BaseModule_perm_trans}.
+
+  Lemma PSubsteps_BaseModule_rewrite m m' o l :
+    BaseModule_perm m m' -> PSubsteps m o l -> PSubsteps m' o l.
+  Proof.
+    intro; inv H; induction 1.
+    - econstructor 1; rewrite <- HRegsPerm; assumption.
+    - econstructor 2; try rewrite <- HRegsPerm; try rewrite <- HRulesPerm; eauto.
+    - econstructor 3; try rewrite <- HRegsPerm; try rewrite <- HMethsPerm; eauto.
+  Qed.
+
+  Lemma PSubsteps_rewrite_all m m' o o' l l' :
+    BaseModule_perm m m' -> o [=] o' -> l [=] l' -> PSubsteps m o l -> PSubsteps m' o' l'.
+  Proof.
+    intros.
+    apply (PSubsteps_BaseModule_rewrite H) in H2.
+    apply (PSubsteps_rewrite_both H0 H1) in H2.
+    assumption.
+  Qed.
+    
+  Global Instance PSubsteps_rewrite' :
+    Proper (@BaseModule_perm ==>
+        @Permutation (string * {x : FullKind & fullType type x}) ==>
+                         @Permutation (FullLabel) ==> iff) (@PSubsteps)| 10.
+  Proof.
+    repeat red; intros; split; intros; eauto using Permutation_sym, BaseModule_perm_sym, PSubsteps_rewrite_all.
+  Qed.
+End PSubsteps_rewrite.
+Section InExec_InCall_perm.
+  Variable f : MethT.
+  
+  Lemma InCall_perm l l' :
+    l [=] l' -> InCall f l  -> InCall f l'.
+    induction 1; intros.
+    - assumption.
+    - apply (InCall_app_iff f (x::nil) l').
+      apply (InCall_app_iff f (x::nil) l) in H0.
+      destruct H0;[left|right; apply IHPermutation];assumption.
+    - apply (InCall_app_iff f (x::y::nil) l).
+      apply (InCall_app_iff f (y::x::nil) l) in H.
+      destruct H;[left;apply (InCall_app_iff f (x::nil) (y::nil)) | right];
+        [apply (InCall_app_iff f (y::nil) (x::nil)) in H; destruct H;[right|left]|];assumption.
+    - apply (IHPermutation2 (IHPermutation1 H1)).
+  Qed.
+
+  Lemma InExec_perm l l' :
+    l [=] l' -> InExec f l -> InExec f l'.
+    induction 1; intros.
+    - assumption.
+    - apply (InExec_app_iff f (x::nil) l').
+      apply (InExec_app_iff f (x::nil) l) in H0.
+      destruct H0;[left|right; apply IHPermutation];assumption.
+    - apply (InExec_app_iff f (x::y::nil) l).
+      apply (InExec_app_iff f (y::x::nil) l) in H.
+      destruct H;[left;apply (InExec_app_iff f (x::nil) (y::nil)) | right];
+        [apply (InExec_app_iff f (y::nil) (x::nil)) in H; destruct H;[right|left]|];assumption.
+    - apply (IHPermutation2 (IHPermutation1 H1)).
+  Qed.
+
+  Global Instance InCall_perm' :
+    Proper (@Permutation (FullLabel) ==> iff) (@InCall f) | 10.
+  Proof.
+    repeat red; intros; specialize (Permutation_sym H) as TMP; eauto using InCall_perm.
+  Qed.
+
+  Global Instance InExec_perm' :
+    Proper (@Permutation (FullLabel) ==> iff) (@InExec f) | 10.
+  Proof.
+    repeat red; intros; specialize (Permutation_sym H) as TMP; eauto using InExec_perm.
+  Qed.
+End InExec_InCall_perm.
+
+Section PStep_rewrite.
+  
+  Lemma MatchingExecCalls_perm1 l1 l2 l3 m:
+    l1 [=] l3 -> MatchingExecCalls l1 l2 m -> MatchingExecCalls l3 l2 m.
+  Proof.
+    repeat intro.
+    specialize (H0 f).
+    apply H0; auto.
+    rewrite H; assumption.
+  Qed.
+
+  Lemma MatchingExecCalls_perm2 l1 l2 l3 m:
+    l2 [=] l3 -> MatchingExecCalls l1 l2 m -> MatchingExecCalls l1 l3 m.
+  Proof.
+    repeat intro.
+    specialize (H0 f).
+    rewrite <- H.
+    apply H0; auto.
+  Qed.
+
+  Lemma MatchingExecCalls_perm l1 l2 l3 l4 m:
+    l1 [=] l3 ->
+    l2 [=] l4 ->
+    MatchingExecCalls l1 l2 m ->
+    MatchingExecCalls l3 l4 m.
+  Proof.
+    intros; eauto using MatchingExecCalls_perm1, MatchingExecCalls_perm2.
+  Qed.
+    
+  Global Instance MatchingExecCalls_perm' :
+    Proper (@Permutation (FullLabel) ==>
+                         @Permutation (FullLabel) ==>
+                         Logic.eq ==>
+                         iff) (@MatchingExecCalls) | 10.
+  Proof.
+    repeat red; split; intros; subst;
+      specialize (Permutation_sym H) as TMP; specialize (Permutation_sym H0) as TMP1;
+        eauto using MatchingExecCalls_perm.
+  Qed.
+  
+  Lemma PStep_rewrite m o1 o2 l1 l2 :
+    (o1 [=] o2) ->
+    (l1 [=] l2) ->
+    PStep m o1 l1 ->
+    PStep m o2 l2.
+  Proof.
+    induction 3.
+    - econstructor 1.
+      apply (PSubsteps_rewrite_regs H).
+      apply (PSubsteps_rewrite_lists H0).
+      assumption.
+      rewrite <- H0.
+      assumption.
+    - econstructor 2; eauto.
+      intros.
+      rewrite <- H0.
+      eapply HHidden; eauto.
+      rewrite H0; assumption.
+    - econstructor 3; eauto.
+      + rewrite <- H; assumption.
+      + rewrite <- H0; assumption.
+  Qed.
+
+  Global Instance Step_perm_rewrite' :
+    Proper (Logic.eq ==> @Permutation (string * {x : FullKind & fullType type x})
+                     ==> @Permutation FullLabel
+                     ==> iff) (@PStep) | 10.
+  repeat red; split; intros; subst;
+    specialize (Permutation_sym H0) as TMP; specialize (Permutation_sym H1) as TMP1;
+      eauto using PStep_rewrite.
+  Qed.
+End PStep_rewrite.
+
+Lemma PSemActionUpdSub o k a reads upds calls ret:
+  @PSemAction o k a reads upds calls ret ->
+  SubList (getKindAttr upds) (getKindAttr o).
+Proof.
+  induction 1; auto;
+    unfold SubList in *; intros;
+      rewrite ?in_app_iff in *.
+  - rewrite HUNewRegs in *.
+    rewrite map_app, in_app_iff in *.
+    destruct H1; firstorder fail.
+  - subst; rewrite HANewRegs in *;firstorder; simpl in *.
+    subst.
+    assumption.
+  - rewrite HUNewRegs in *.
+    rewrite map_app, in_app_iff in *.
+    destruct H1; intuition.
+  - rewrite HUNewRegs in *.
+    rewrite map_app, in_app_iff in *.
+    destruct H1; intuition.
+  - subst; simpl in *; intuition.
+Qed.
+
+Lemma PSemActionExpandRegs o k a reads upds calls ret:
+  @PSemAction o k a reads upds calls ret ->
+  forall o', SubList reads o' ->
+             SubList (getKindAttr upds) (getKindAttr o') ->
+             @PSemAction o' k a reads upds calls ret.
+Proof.
+  intros.
+  induction H; try solve [econstructor; auto].
+  - subst.
+    specialize (IHPSemAction H0).
+    econstructor; eauto.
+  - rewrite HUReadRegs in *; rewrite HUNewRegs in *.
+    apply SubList_app_l in H0; dest.
+    rewrite map_app in *.
+    apply SubList_app_l in H1; dest.
+    specialize (IHPSemAction1 H0 H1).
+    specialize (IHPSemAction2 H3 H4).
+    econstructor; eauto.
+  - rewrite HNewReads in *.
+    apply SubList_cons in H0; dest.
+    specialize (IHPSemAction H2 H1).
+    econstructor; eauto.
+  - rewrite HANewRegs in *.
+    simpl in *.
+    apply SubList_cons in H1; dest.
+    specialize (IHPSemAction H0 H2).
+    econstructor; eauto.
+  - rewrite HUReadRegs in *; rewrite HUNewRegs in *.
+    apply SubList_app_l in H0; dest.
+    rewrite map_app in *.
+    apply SubList_app_l in H1; dest.
+    specialize (IHPSemAction1 H0 H1).
+    specialize (IHPSemAction2 H3 H4).
+    econstructor; eauto.
+  - rewrite HUReadRegs in *; rewrite HUNewRegs in *.
+    apply SubList_app_l in H0; dest.
+    rewrite map_app in *.
+    apply SubList_app_l in H1; dest.
+    specialize (IHPSemAction1 H0 H1).
+    specialize (IHPSemAction2 H3 H4).
+    econstructor 8; eauto.
+Qed.
+
+Lemma PSubsteps_upd_SubList_key m o l:
+  PSubsteps m o l ->
+  forall x s v, In x (map fst l) ->
+                In (s, v) x ->
+                In s (map fst (getRegisters m)).
+Proof.
+  induction 1; intros.
+  - simpl in *; tauto.
+  - subst; rewrite HLabel in H0.
+    destruct H0; subst; simpl in *.
+    + apply (in_map (fun x => (fst x, projT1 (snd x)))) in H1; simpl in *.
+      specialize (HUpdGood _ H1).
+      apply (in_map fst) in HUpdGood.
+      rewrite map_map in HUpdGood.
+      simpl in *.
+      setoid_rewrite (functional_extensionality (fun x => fst x) fst) in HUpdGood; auto.
+    + eapply IHPSubsteps; eauto.
+  - subst; rewrite HLabel in H0.
+    destruct H0; subst; simpl in *.
+    + apply (in_map (fun x => (fst x, projT1 (snd x)))) in H1; simpl in *.
+      specialize (HUpdGood _ H1).
+      apply (in_map fst) in HUpdGood.
+      rewrite map_map in HUpdGood.
+      simpl in *.
+      setoid_rewrite (functional_extensionality (fun x => fst x) fst) in HUpdGood; auto.
+    + eapply IHPSubsteps; eauto.
+Qed.
+
+Lemma PSubsteps_upd_In m o l:
+  PSubsteps m o l ->
+  forall x, In x (map fst l) ->
+            forall s: string, In s (map fst x) ->
+                              In s (map fst (getRegisters m)).
+Proof.
+  intros.
+  rewrite in_map_iff in H1; dest; subst.
+  destruct x0; simpl.
+  eapply PSubsteps_upd_SubList_key; eauto.
+Qed.
+
+Lemma PSubsteps_combine m1 o1 l1:
+  PSubsteps m1 o1 l1 ->
+  forall m2 o2 l2  (DisjRegs: DisjKey (getRegisters m1) (getRegisters m2)) (DisjMeths: DisjKey (getMethods m1) (getMethods m2))
+         (HOneRle: forall x1 x2, In x1 l1 -> In x2 l2 -> match fst (snd x1), fst (snd x2) with
+                                                         | Rle _, Rle _ => False
+                                                         | _, _ => True
+                                                         end)
+         (HNoCall: forall x, InCall x l1 -> InCall x l2 -> False),
+    PSubsteps m2 o2 l2 ->
+    PSubsteps (BaseMod (getRegisters m1 ++ getRegisters m2) (getRules m1 ++ getRules m2) (getMethods m1 ++ getMethods m2)) (o1 ++ o2) (l1 ++ l2).
+Proof.
+  induction 1; intros.
+  - induction H; simpl in *.
+    + constructor 1; auto; simpl.
+      rewrite ?map_app; rewrite HRegs0; rewrite HRegs. reflexivity.
+    + econstructor 2; eauto; simpl; rewrite ?map_app; try congruence.
+      * rewrite HRegs; rewrite HRegs0; reflexivity.
+      * rewrite in_app_iff; right; eassumption.
+      * specialize (PSemAction_SemAction HPAction) as TMP; dest.
+        pose proof (SemActionReadsSub (BaseMod (getRegisters m1 ++ getRegisters m2) (getRules m1 ++ getRules m2) (getMethods m1 ++ getMethods m2)) H3).
+        pose proof (SemActionUpdSub H3).
+        eapply PSemActionExpandRegs; eauto; unfold SubList in *; intros; rewrite ?map_app, ?in_app_iff; right.
+        -- eapply H4; rewrite <- H0; eauto.
+        -- eapply H5; rewrite <- H1; eauto.
+      * unfold SubList in *; intros.
+        rewrite in_app_iff; right; eapply HReadsGood; eauto.
+      * unfold SubList in *; intros.
+        rewrite in_app_iff; right; eapply HUpdGood; eauto.
+      * eapply IHPSubsteps; intros;
+          unfold InCall in *; simpl in *; dest; tauto.
+    + econstructor 3; eauto; simpl; rewrite ?map_app; try congruence.
+      * rewrite HRegs; rewrite HRegs0; reflexivity.
+      * rewrite in_app_iff; right; eassumption.
+      * specialize (PSemAction_SemAction HPAction) as TMP; dest.
+        pose proof (SemActionReadsSub (BaseMod (getRegisters m1 ++ getRegisters m2) (getRules m1 ++ getRules m2) (getMethods m1 ++ getMethods m2)) H3).
+        pose proof (SemActionUpdSub H3).
+        eapply PSemActionExpandRegs; eauto; unfold SubList in *; intros; rewrite ?map_app, ?in_app_iff; right.
+        -- eapply H4; rewrite <- H0; eauto.
+        -- eapply H5; rewrite <- H1; eauto.
+      * unfold SubList in *; intros.
+        rewrite in_app_iff; right; eapply HReadsGood; eauto.
+      * unfold SubList in *; intros.
+        rewrite in_app_iff; right; eapply HUpdGood; eauto.
+      * eapply IHPSubsteps; intros;
+          unfold InCall in *; simpl in *; dest; tauto.
+  - subst; simpl; rewrite HLabel.
+    assert (sth_else: forall x1 x2, In x1 ls -> In x2 l2 -> match fst (snd x1), fst (snd x2) with
+                                                            | Rle _, Rle _ => False
+                                                            | _, _ => True
+                                                            end);[intros x1 x2; specialize (HOneRle x1 x2); rewrite HLabel in *; clear - HOneRle; firstorder fail|].
+    assert (sth2_else: forall x, InCall x ls -> InCall x l2 -> False);[intros x; specialize (HNoCall0 x); rewrite HLabel in *;clear - HNoCall0; firstorder fail|].
+    specialize (IHPSubsteps _ _ _ DisjRegs DisjMeths sth_else sth2_else H0).
+    simpl; econstructor 2; eauto; simpl; rewrite ?map_app; try congruence.
+    + inv H0; rewrite HRegs; rewrite HRegs0; reflexivity.
+    + rewrite in_app_iff; left; eassumption.
+    + specialize (PSemAction_SemAction HPAction) as TMP;dest.
+      pose proof (SemActionReadsSub (BaseMod (getRegisters m1 ++ getRegisters m2) (getRules m1 ++ getRules m2) (getMethods m1 ++ getMethods m2)) H4).
+      pose proof (SemActionUpdSub H4).
+      eapply PSemActionExpandRegs; eauto; unfold SubList in *; intros; rewrite ?map_app, ?in_app_iff; left.
+      * eapply H5; rewrite <- H1; eauto.
+      * eapply H6; rewrite <- H2; eauto.
+    + unfold SubList in *; intros.
+      rewrite in_app_iff; left; eapply HReadsGood; eauto.
+    + unfold SubList in *; intros.
+      rewrite in_app_iff; left; eapply HUpdGood; eauto.
+    + intros.
+      rewrite in_app_iff in *.
+      destruct H1; [eapply HDisjRegs; eauto| ].
+      rewrite DisjKeyWeak_same by apply string_dec; intro; intros.
+      rewrite in_map_iff in H2; dest; subst.   
+      pose proof (PSubsteps_upd_In H0 _ (in_map fst _ _ H1) _ (in_map fst _ _ H4)).
+      apply (SubList_map fst) in HUpdGood.
+      rewrite ?map_map in *; simpl in *.
+      rewrite ?(functional_extensionality (fun x => fst x) fst) in HUpdGood by tauto.
+      setoid_rewrite (functional_extensionality (fun x => fst x) fst) in HUpdGood; [|tauto].
+      specialize (HUpdGood _ H3).
+      clear - H2 DisjRegs HUpdGood; firstorder fail.
+    + intros.
+      rewrite in_app_iff in *.
+      destruct H1; [eapply HNoRle; eauto| ].
+      unfold SubList in *.
+      specialize (HOneRle (u, (Rle rn, cs)) x); rewrite HLabel in HOneRle.
+      specialize (HOneRle (or_introl eq_refl) H1); simpl in *; assumption.
+    + intros.
+      rewrite InCall_app_iff in *.
+      destruct H2; [eapply HNoCall; eauto|].
+      eapply HNoCall0; eauto.
+      rewrite HLabel.
+      unfold InCall.
+      eexists; split; simpl; eauto.
+  - subst; simpl.
+    assert (sth_else: forall x1 x2, In x1 ls -> In x2 l2 -> match fst (snd x1), fst (snd x2) with
+                                                            | Rle _, Rle _ => False
+                                                            | _, _ => True
+                                                            end);[intros;specialize (HOneRle x1 x2);rewrite HLabel in * ; firstorder fail|].
+    assert (sth2_else: forall x, InCall x ls -> InCall x l2 -> False);[intros; specialize (HNoCall0 x); rewrite HLabel in *; firstorder fail|].
+    specialize (IHPSubsteps _ _ _ DisjRegs DisjMeths sth_else sth2_else H0).
+    rewrite HLabel;simpl; econstructor 3; eauto; simpl; rewrite ?map_app; try congruence.
+    + inv H0;rewrite HRegs; rewrite HRegs0; reflexivity.
+    + rewrite in_app_iff; left; eassumption.
+    + specialize (PSemAction_SemAction HPAction) as TMP; dest.
+      pose proof (SemActionReadsSub (BaseMod (getRegisters m1 ++ getRegisters m2) (getRules m1 ++ getRules m2) (getMethods m1 ++ getMethods m2)) H4).
+      pose proof (SemActionUpdSub H4).
+      eapply PSemActionExpandRegs; eauto; unfold SubList in *; intros; rewrite ?map_app, ?in_app_iff; left.
+      * eapply H5; rewrite <- H1; eauto.
+      * eapply H6; rewrite <- H2; eauto.
+    + unfold SubList in *; intros.
+      rewrite in_app_iff; left; eapply HReadsGood; eauto.
+    + unfold SubList in *; intros.
+      rewrite in_app_iff; left; eapply HUpdGood; eauto.
+    + intros.
+      rewrite in_app_iff in *.
+      destruct H1; [eapply HDisjRegs; eauto| ].
+      rewrite DisjKeyWeak_same by apply string_dec; intro; intros.
+      rewrite in_map_iff in H2; dest; subst.
+      pose proof (PSubsteps_upd_In H0 _ (in_map fst _ _ H1) _ (in_map fst _ _ H4)).
+      apply (SubList_map fst) in HUpdGood.
+      rewrite ?map_map in *; simpl in *.
+      rewrite ?(functional_extensionality (fun x => fst x) fst) in HUpdGood by tauto.
+      setoid_rewrite (functional_extensionality (fun x => fst x) fst) in HUpdGood; [|tauto].
+      specialize (HUpdGood _ H3).
+      clear - H2 DisjRegs HUpdGood; firstorder fail.
+    + intros.
+      rewrite InCall_app_iff in *.
+      destruct H2; [eapply HNoCall; eauto|].
+      eapply HNoCall0; eauto.
+      unfold InCall.
+      eexists; rewrite HLabel;split; simpl; eauto.
+Qed.
+
+Corollary PStep_meth_InExec m o l :
+  PStep m o l ->
+  forall f : MethT,
+    InExec f l -> In (fst f) (map fst (getAllMethods m)).
+Proof.
+  intros.
+  apply PStep_Step in H; dest.
+  eapply (Step_meth_InExec H3 f).
+  apply (List_FullLabel_perm_InExec_rewrite f H2); assumption.
+Qed.
+
+Lemma PStep_substitute' m o l:
+  PStep m o l -> forall (HWfMod: WfMod m), PStepSubstitute m o l.
+Proof.
+  unfold StepSubstitute.
+  induction 1; auto; simpl; intros; dest; unfold MatchingExecCalls in *; simpl in *.
+  - repeat split.
+    clear HMatching.
+    induction HPSubsteps.
+    + econstructor 1; eauto.
+    + econstructor 2; eauto.
+    + econstructor 3; eauto.
+    + simpl; tauto.
+    + specialize (HMatching f); tauto.
+    + simpl in *; tauto.
+  - inv HWfMod.
+    specialize (IHPStep HWf); unfold PStepSubstitute in IHPStep; dest.
+    repeat split; auto.
+    + specialize (H1 f); tauto.
+    + intros.
+      destruct H4; simpl in *; subst.
+      -- apply HHidden; auto.
+      -- apply H2; auto.
+  - inv HWfMod.
+    specialize (IHPStep1 HWf1).
+    specialize (IHPStep2 HWf2).
+    unfold PStepSubstitute in *; dest.
+    subst; repeat split; auto.
+    + pose proof (PSubsteps_combine H4  HDisjRegs HDisjMeths HNoRle HNoCall H1 (m2 := BaseMod (getAllRegisters m2) _ _)).
+      simpl in *.
+      rewrite HLabels; rewrite HRegs.
+      assumption.
+    + rewrite HLabels in *.
+      unfold MatchingExecCalls in *; simpl in *.
+      rewrite ?InExec_app_iff, ?InCall_app_iff, ?map_app, ?in_app_iff in *.
+      repeat match goal with
+             | H: forall x: MethT, _ |- _ => specialize (H f)
+             end; tauto.
+    + intros.
+      rewrite HLabels in *.
+      unfold MatchingExecCalls in *; simpl in *.
+      rewrite ?InExec_app_iff, ?InCall_app_iff, ?map_app, ?in_app_iff in *.
+      repeat match goal with
+             | H: forall x: string, _ |- _ => specialize (H s)
+             | H: forall x: MethT, _ |- _ => specialize (H (s, v))
+             end.
+      specialize (H6 v); specialize (H3 v).
+      destruct H7, H8, H9; try tauto.
+      * pose proof (PStep_meth_InExec H0 _ H9); simpl in *.
+        clear - HDisjMeths H7 H10; firstorder fail.
+      * pose proof (WfMod_Hidden HWf2 s H8).
+        clear - HDisjMeths H7 H10; firstorder fail.
+      * pose proof (WfMod_Hidden HWf2 s H8).
+        clear - HDisjMeths H7 H10; firstorder fail.
+      * pose proof (WfMod_Hidden HWf1 s H8).
+        clear - HDisjMeths H7 H10; firstorder fail.
+      * pose proof (WfMod_Hidden HWf1 s H8).
+        clear - HDisjMeths H7 H10; firstorder fail.
+      * pose proof (PStep_meth_InExec H _ H9); simpl in *.
+        clear - HDisjMeths H7 H10; firstorder fail.
+Qed.
+
+Lemma PStepSubstitute_flatten m o l (HWfMod: WfMod m):
+  PStep (flatten m) o l <-> PStepSubstitute m o l.
+Proof.
+  unfold flatten, getFlat, PStepSubstitute.
+  split; intros.
+  - induction (getHidden m).
+    + simpl in *.
+      inv H.
+      split; [auto| split; [auto| intros; tauto]].
+    + simpl in *.
+      inv H.
+      specialize (IHl0 HPStep); dest.
+      split; [auto| split; [auto| intros]].
+      rewrite createHide_Meths in *; simpl in *.
+      destruct H3; [subst |clear - H1 H2 H3 H4; firstorder fail].
+      firstorder fail.
+  - induction (getHidden m); simpl; auto; dest.
+    + constructor; auto.
+    + assert (sth: PStep (createHide (BaseMod (getAllRegisters m) (getAllRules m) (getAllMethods m)) l0) o l) by firstorder fail.
+      assert (sth2: forall v, In a (map fst (getAllMethods m)) -> InExec (a, v) l -> InCall (a, v) l) by firstorder fail.
+      constructor; auto.
+      rewrite createHide_Meths.
+      auto.
+Qed.
+
+Lemma PStep_substitute m o l (HWfMod: WfMod m):
+  PStep m o l -> PStep (flatten m) o l.
+Proof.
+  intros Stp.
+  apply PStep_substitute' in Stp; auto.
+  rewrite PStepSubstitute_flatten in *; auto.
+Qed.
+
+Lemma splitRegs o m1 m2 (DisjRegisters: DisjKey (getRegisters m1) (getRegisters m2)):
+  getKindAttr o [=] getKindAttr (getRegisters m1 ++ getRegisters m2) ->
+  getKindAttr (filter (fun x : string * {x : FullKind & fullType type x} => getBool (in_dec string_dec (fst x) (map fst (getRegisters m1)))) o) [=] getKindAttr (getRegisters m1).
+Proof.
+  intros HRegs.
+  rewrite map_app in *.
+  pose proof (filter_map_simple (fun x: string * {x: FullKind & fullType type x} => (fst x, projT1 (snd x)))
+                                (fun x => getBool (in_dec string_dec (fst x) (map fst (getRegisters m1)))) o) as sth.
+  simpl in sth.
+  setoid_rewrite <- sth.
+  setoid_rewrite HRegs.
+  rewrite filter_app.
+  setoid_rewrite filter_false_list at 2.
+  - rewrite filter_true_list at 1.
+    + rewrite app_nil_r; auto.
+    + intros.
+      apply (in_map fst) in H.
+      rewrite map_map in H.
+      simpl in *.
+      setoid_rewrite (functional_extensionality (fun x => fst x) fst) in H; try tauto.
+      destruct (in_dec string_dec (fst a) (map fst (getRegisters m1))); auto.
+  - intros.
+    apply (in_map fst) in H.
+    rewrite map_map in H.
+    simpl in *.
+    setoid_rewrite (functional_extensionality (fun x => fst x) fst) in H; try tauto.
+    destruct (in_dec string_dec (fst a) (map fst (getRegisters m1))); auto.
+    specialize (DisjRegisters (fst a)).
+    tauto.
+Qed.
+
+Global Instance BaseModuleFilter_rewrite' :
+  Proper (Logic.eq ==> @Permutation (FullLabel) ==> @Permutation (FullLabel)) (@ModuleFilterLabels) | 10.
+Proof.
+  unfold ModuleFilterLabels; repeat red; intros; rewrite H, H0; reflexivity.
+Qed.
+
+Lemma WfActionT_ReadsWellDefined_perm : forall (k : Kind)(a : ActionT type k)(retl : type k)
+                                          (m1 : BaseModule)(o readRegs newRegs : RegsT)(calls : MethsT),
+    WfActionT m1 a ->
+    PSemAction o a readRegs newRegs calls retl ->
+    SubList (getKindAttr readRegs) (getKindAttr (getRegisters m1)).
+Proof.
+  intros.
+  apply (PSemAction_SemAction) in H0; dest.
+  rewrite H0.
+  eapply (WfActionT_ReadsWellDefined H H3); eauto.
+Qed.
+
+Lemma WfActionT_WritesWellDefined_perm : forall (k : Kind)(a : ActionT type k)(retl : type k)
+                                           (m1 : BaseModule)(o readRegs newRegs : RegsT)(calls : MethsT),
+    WfActionT m1 a ->
+    PSemAction o a readRegs newRegs calls retl ->
+    SubList (getKindAttr newRegs) (getKindAttr (getRegisters m1)).
+Proof.
+  intros.
+  apply (PSemAction_SemAction) in H0; dest.
+  rewrite H1.
+  eapply (WfActionT_WritesWellDefined); eauto.
+Qed.
+
+Lemma WfActionT_PSemAction : forall (k : Kind)(a : ActionT type k)(retl : type k)
+                                   (m1 : BaseModule)(o readRegs newRegs : RegsT)(calls : MethsT),
+    WfActionT m1 a ->
+    NoDup (map fst o) ->
+    PSemAction o a readRegs newRegs calls retl ->
+    (forall (o1 : RegsT),
+        SubList o1 o ->
+        getKindAttr o1 [=] getKindAttr (getRegisters m1) ->
+        PSemAction o1 a readRegs newRegs calls retl).
+  induction 3; intro; subst; inversion H; EqDep_subst.
+  - intros TMP1 TMP2; specialize (IHPSemAction (H4 mret) o1 TMP1 TMP2).
+    econstructor 1; eauto.
+  - intros TMP1 TMP2; specialize (IHPSemAction (H4) o1 TMP1 TMP2).
+    econstructor 2; eauto.
+  - intros TMP1 TMP2; specialize (IHPSemAction1 (H4) o1 TMP1 TMP2); specialize (IHPSemAction2 (H6 v) o1 TMP1 TMP2).
+    econstructor 3; eauto.
+  - intros TMP1 TMP2; specialize (IHPSemAction (H4 valueV) o1 TMP1 TMP2).
+    econstructor 4; eauto.
+  - intros TMP1 TMP2; specialize (IHPSemAction (H5 regV) o1 TMP1 TMP2).
+    econstructor 5; eauto.
+    apply (KeyRefinement (r, existT (fullType type) regT regV) H0 TMP1 HRegVal).
+    rewrite <- TMP2 in H7; apply (in_map fst) in H7; specialize (GKA_fst (A:=string)(fullType type) o1); intro.
+    simpl in *.
+    setoid_rewrite H2; assumption.
+  - intros TMP1 TMP2; specialize (IHPSemAction H5 o1 TMP1 TMP2).
+    econstructor 6; eauto.
+    rewrite TMP2; assumption.
+  - intros TMP1 TMP2; specialize (IHPSemAction1 H8 o1 TMP1 TMP2); specialize (IHPSemAction2 (H5 r1) o1 TMP1 TMP2).
+    econstructor 7; eauto.
+  - intros TMP1 TMP2; specialize (IHPSemAction1 H9 o1 TMP1 TMP2); specialize (IHPSemAction2 (H5 r1) o1 TMP1 TMP2).
+    econstructor 8; eauto.
+  - intros TMP1 TMP2; specialize (IHPSemAction H4 o1 TMP1 TMP2).
+    econstructor 9; eauto.
+  - intros TMP1 TMP2; specialize (IHPSemAction H4 o1 TMP1 TMP2).
+    econstructor 10; eauto.
+  - intros; econstructor 11; eauto.
+Qed.
+
+Lemma papp_sublist_l : forall {A : Type} (l1 l2 l : list A),
+    l [=] l1++l2 -> SubList l1 l.
+Proof.
+  repeat intro.
+  rewrite H.
+  apply (in_app_iff l1 l2 x); left; assumption.
+Qed.
+
+Lemma papp_sublist_r : forall {A : Type} (l1 l2 l : list A),
+    l [=] l1++l2 -> SubList l2 l.
+Proof.
+  repeat intro.
+  rewrite H.
+  apply (in_app_iff l1 l2 x); right; assumption.
+Qed.
+
+Section SplitSubsteps.
+  Variable m1 m2: BaseModule.
+  Variable DisjRegs: DisjKey (getRegisters m1) (getRegisters m2).
+  Variable DisjRules: DisjKey (getRules m1) (getRules m2).
+  Variable DisjMeths: DisjKey (getMethods m1) (getMethods m2).
+
+  Variable WfMod1: WfBaseMod m1.
+  Variable WfMod2: WfBaseMod m2.
+  
+  Lemma pfilter_perm o l :
+    PSubsteps (concatFlat m1 m2) o l ->
+    l [=] ((ModuleFilterLabels m1 l)++(ModuleFilterLabels m2 l)).
+  Proof.   
+    induction 1; subst.
+    - simpl; apply Permutation_refl.
+    - unfold ModuleFilterLabels; setoid_rewrite HLabel; fold (ModuleFilterLabels m1 ((u, (Rle rn, cs))::ls));
+      fold (ModuleFilterLabels m2 ((u, (Rle rn, cs))::ls)). apply in_app_iff in HInRules.
+      destruct HInRules as [HInRules | HInRules]; rewrite (InRules_Filter _ _ _ _ _ _ HInRules).
+      + destruct (DisjRules rn).
+        * generalize (in_map_iff fst (getRules m1) rn). intro TMP; destruct TMP as [L R];clear L.
+          assert (exists x, fst x = rn /\ In x (getRules m1));[exists (rn, rb); auto| specialize (R H1); contradiction].
+        * rewrite (NotInRules_Filter _ _ _ _ _ H0).
+          constructor. assumption.
+      + destruct (DisjRules rn).
+        * rewrite (NotInRules_Filter _ _ _ _ _ H0).
+          apply (Permutation_cons_app _ _ _ IHPSubsteps).
+        * generalize (in_map_iff fst (getRules m2) rn). intro TMP; destruct TMP as [L R];clear L.
+          assert (exists x, fst x = rn /\ In x (getRules m2));[exists (rn, rb); auto | specialize (R H1); contradiction].
+    - apply in_app_iff in HInMeths.
+      unfold ModuleFilterLabels; rewrite HLabel; fold (ModuleFilterLabels m1 ( (u, (Meth (fn, existT SignT (projT1 fb) (argV, retV)), cs))::ls));
+        fold (ModuleFilterLabels m2 ((u, (Meth (fn, existT SignT (projT1 fb) (argV, retV)), cs))::ls));
+      destruct HInMeths as [HInMeths | HInMeths]; rewrite (InMethods_Filter _ _ _ _ _ _ _ _ HInMeths).
+      + destruct (DisjMeths fn).
+        * generalize (in_map_iff fst (getMethods m1) fn). intro TMP; destruct TMP as [L R]; clear L.
+          assert (exists x, fst x = fn /\ In x (getMethods m1)); [exists (fn, fb); auto| specialize (R H1); contradiction].
+        * rewrite (NotInMethods_Filter _ _ _ _ _ _ _ _ H0).
+          constructor. assumption.
+      + destruct (DisjMeths fn).
+        * rewrite (NotInMethods_Filter _ _ _ _ _ _ _ _ H0).
+          apply (Permutation_cons_app _ _ _ IHPSubsteps).
+        * generalize (in_map_iff fst (getMethods m2) fn). intro TMP; destruct TMP as [L R]; clear L.
+          assert (exists x, fst x = fn /\ In x (getMethods m2)); [exists (fn, fb); auto| specialize (R H1); contradiction].
+  Qed.
+
+  Lemma split_f A B (f : A -> B) :
+    forall (ls : list A) (l1 l2 : list B),
+      map f ls [=] l1 ++ l2 ->
+      (exists (ls1 ls2 : list A),
+          (ls [=] ls1++ls2) /\
+          (map f ls1 [=] l1) /\
+          (map f ls2 [=] l2)).
+  Proof.
+    induction ls; intros.
+    - exists nil, nil.
+      apply (Permutation_nil) in H; destruct (app_eq_nil _ _ H).
+      repeat split.
+      + reflexivity.
+      + rewrite H0; reflexivity.
+      + rewrite H1; reflexivity.
+    - assert (In (f a) (map f (a::ls)));[left; reflexivity|].
+      rewrite H in H0.
+      destruct (in_app_or _ _ _ H0).
+      + specialize (in_split _ _ H1) as TMP; dest.
+        rewrite H2 in H; simpl in H.
+        rewrite <- app_assoc in H.
+        specialize (Permutation_cons_app_inv (l:=(map f ls)) x (x0++l2) H) as TMP.
+        rewrite app_assoc in TMP.
+        specialize (IHls (x ++ x0) (l2) TMP) as TMP2; dest.
+        exists (a::x1), x2.
+        repeat split.
+        * simpl; constructor; auto.
+        * simpl; rewrite H2.
+          apply Permutation_cons_app.
+          assumption.
+        * assumption.
+      + specialize (in_split _ _ H1) as TMP; dest.
+        rewrite H2 in H; simpl in H.
+        rewrite app_assoc in H.
+        specialize (Permutation_cons_app_inv (l:=(map f ls)) (l1++x) x0 H) as TMP.
+        rewrite <- app_assoc in TMP.
+        specialize (IHls (l1) (x++x0) TMP) as TMP2; dest.
+        exists (x1), (a::x2).
+        repeat split.
+        * apply Permutation_cons_app; assumption.
+        * assumption.
+        * simpl; rewrite H2.
+          apply Permutation_cons_app.
+          assumption.
+  Qed.
+  
+  Lemma split_PSubsteps1 o l:
+    NoDup (map fst (getRegisters m1)) ->
+    NoDup (map fst (getRegisters m2)) ->
+    PSubsteps (concatFlat m1 m2) o l ->
+    (exists o1 o2, getKindAttr o1 [=] getKindAttr (getRegisters m1) /\
+                   getKindAttr o2 [=] getKindAttr (getRegisters m2) /\
+                   o [=] o1++o2 /\
+                   PSubsteps m1 o1 (ModuleFilterLabels m1 l) /\
+                   PSubsteps m2 o2 (ModuleFilterLabels m2 l)).
+  Proof.
+    unfold concatFlat; induction 3; simpl in *.
+    - rewrite map_app in *; apply split_f in HRegs; dest.
+      exists x, x0;split;[|split;[|split;[|split;[constructor|constructor]]]];assumption.
+    - rewrite map_app in *;apply in_app_iff in HInRules; specialize (DisjRules rn).
+      assert (NoDup (map fst o));[setoid_rewrite GKA_fst;setoid_rewrite HRegs; rewrite <- map_app; rewrite <- GKA_fst; apply (NoDupKey_Expand H H0 DisjRegs)|].
+      destruct HInRules as [HInRules|HInRules];generalize (in_map fst _ _ HInRules);destruct DisjRules;try contradiction.
+      + subst; dest; exists x, x0;split;[|split;[|split;[|split]]];auto.
+        rewrite HLabel in *.
+        rewrite (InRules_Filter _ _ _ _ _ _ HInRules).
+        destruct WfMod1 as [WfMod_Rle1 WfMod_Meth1];destruct WfMod2 as [WfMod_Rle2 WfMod_Meth2];
+          specialize (WfActionT_ReadsWellDefined_perm (WfMod_Rle1 _ HInRules) HPAction) as Reads_sublist; specialize (WfActionT_WritesWellDefined_perm (WfMod_Rle1 _ HInRules) HPAction) as Writes_sublist.
+        constructor 2 with (rn:= rn)(rb:=rb)(reads:=reads)(u:=u)(cs:=cs)(ls:=(ModuleFilterLabels m1 ls)); auto.
+        * specialize (papp_sublist_l _ _ H6) as SL_o_x.
+          specialize (WfMod_Rle1 (rn, rb) HInRules); specialize (WfActionT_PSemAction WfMod_Rle1 H2 HPAction SL_o_x H4).
+          simpl; auto.
+        * unfold ModuleFilterLabels;intros;apply HDisjRegs;
+            destruct (filter_In (BaseModuleFilter m1) x1 ls) as [L R];
+            destruct (L H10);assumption.
+        * intros; apply HNoRle;
+            destruct (filter_In (BaseModuleFilter m1) x1 ls) as [L R];
+            destruct (L H10);assumption.
+        * intros; apply (HNoCall c H10). destruct H11 as [x1 [L R]];exists x1;split;[|assumption].
+          destruct (filter_In (BaseModuleFilter m1) x1 ls) as [L1 R1]; destruct (L1 L); assumption.
+        * rewrite HLabel,(NotInRules_Filter _ _ _ _ _ H3); assumption.
+      + subst; dest; exists x, x0; split;[|split;[|split;[|split]]];auto.
+        rewrite HLabel,(NotInRules_Filter _ _ _ _ _ H3); assumption.
+        rewrite HLabel,(InRules_Filter _ _ _ _ _ _ HInRules).
+        destruct WfMod1 as [WfMod_Rle1 WfMod_Meth1];destruct WfMod2 as [WfMod_Rle2 WfMod_Meth2];
+          specialize (WfActionT_ReadsWellDefined_perm (WfMod_Rle2 _ HInRules) HPAction) as Reads_sublist; specialize (WfActionT_WritesWellDefined_perm (WfMod_Rle2 _ HInRules) HPAction) as Writes_sublist.
+        constructor 2 with (rn:= rn)(rb:=rb)(reads:=reads)(u:=u)(cs:=cs)(ls:=(ModuleFilterLabels m2 ls)); auto.
+        * specialize (papp_sublist_r _ _ H6) as SL_o_x.
+          specialize (WfMod_Rle2 (rn, rb) HInRules); specialize (WfActionT_PSemAction WfMod_Rle2 H2 HPAction SL_o_x H5).
+          simpl; auto.
+        * unfold ModuleFilterLabels;intros;apply HDisjRegs;
+            destruct (filter_In (BaseModuleFilter m2) x1 ls) as [L R];
+            destruct (L H10);assumption.
+        * intros; apply HNoRle;
+            destruct (filter_In (BaseModuleFilter m2) x1 ls) as [L R];
+            destruct (L H10);assumption.
+        * intros; apply (HNoCall c H10). destruct H11 as [x1 [L R]];exists x1;split;[|assumption].
+          destruct (filter_In (BaseModuleFilter m2) x1 ls) as [L1 R1]; destruct (L1 L); assumption.
+    - rewrite map_app in *;apply in_app_iff in HInMeths; specialize (DisjMeths fn).
+      assert (NoDup (map fst o));[setoid_rewrite GKA_fst;setoid_rewrite HRegs; rewrite <- map_app; rewrite <- GKA_fst; apply (NoDupKey_Expand H H0 DisjRegs)|].
+      destruct HInMeths as [HInMeths|HInMeths];generalize (in_map fst _ _ HInMeths);destruct DisjMeths;try contradiction;intros.
+      + subst; dest; exists x, x0;split;[|split;[|split;[|split]]];auto.
+        * rewrite HLabel,(InMethods_Filter _ _ _ _ _ _ _ _ HInMeths).
+          destruct WfMod1 as [WfMod_Rle1 WfMod_Meth1];destruct WfMod2 as [WfMod_Rle2 WfMod_Meth2]; specialize (WfActionT_ReadsWellDefined_perm (WfMod_Meth1 (fn, fb) HInMeths argV) HPAction) as Reads_sublist; specialize (WfActionT_WritesWellDefined_perm (WfMod_Meth1 (fn, fb) HInMeths argV) HPAction) as Writes_sublist.
+          constructor 3 with (fn:=fn)(fb:=fb)(reads:=reads)(u:=u)(cs:=cs)(argV:=argV)(retV:=retV)(ls:=(ModuleFilterLabels m1 ls)); auto.
+          -- specialize (papp_sublist_l _ _ H7) as SL_o_x.
+             specialize (WfMod_Meth1 (fn, fb) HInMeths argV); specialize (WfActionT_PSemAction WfMod_Meth1 H2 HPAction SL_o_x H5).
+             simpl; auto.
+          -- intros; apply HDisjRegs;
+               destruct (filter_In (BaseModuleFilter m1) x1 ls) as [L R];
+               destruct (L H10); assumption.
+          -- intros; apply (HNoCall c H10). destruct H11 as [x1 [L R]];exists x1;split;[|assumption].
+             destruct (filter_In (BaseModuleFilter m1) x1 ls) as [L1 R1]; destruct (L1 L); assumption.
+        * rewrite HLabel,(NotInMethods_Filter _ _ _ _ _ _ _ _ H3); assumption.
+      + subst; dest; exists x, x0;split;[|split;[|split;[|split]]]; auto.
+        * rewrite HLabel,(NotInMethods_Filter _ _ _ _ _ _ _ _ H3); assumption.
+        * rewrite HLabel,(InMethods_Filter _ _ _ _ _ _ _ _ HInMeths).
+          destruct WfMod1 as [WfMod_Rle1 WfMod_Meth1];destruct WfMod2 as [WfMod_Rle2 WfMod_Meth2];
+            specialize (WfActionT_ReadsWellDefined_perm (WfMod_Meth2 (fn, fb) HInMeths argV) HPAction) as Reads_sublist;
+            specialize (WfActionT_WritesWellDefined_perm (WfMod_Meth2 (fn, fb) HInMeths argV) HPAction) as Writes_sublist.
+          constructor 3 with (fn:=fn)(fb:=fb)(reads:=reads)(u:=u)(cs:=cs)(argV:=argV)(retV:=retV)(ls:=(ModuleFilterLabels m2 ls)); auto.
+          -- specialize (papp_sublist_r _ _ H7) as SL_o_x.
+             specialize (WfMod_Meth2 (fn, fb) HInMeths argV); specialize (WfActionT_PSemAction WfMod_Meth2 H2 HPAction SL_o_x H6).
+             simpl; auto.
+          -- intros; apply HDisjRegs;
+               destruct (filter_In (BaseModuleFilter m2) x1 ls) as [L R];
+               destruct (L H10); assumption.
+          -- intros; apply (HNoCall c H10). destruct H11 as [x1 [L R]];exists x1;split;[|assumption].
+             destruct (filter_In (BaseModuleFilter m2) x1 ls) as [L1 R1]; destruct (L1 L); assumption.
+  Qed.
+  
+  Lemma split_Substeps2 o l:
+    PSubsteps (concatFlat m1 m2) o l ->
+      (forall x y : FullLabel,
+          In x (ModuleFilterLabels m1 l) ->
+          In y (ModuleFilterLabels m2 l) ->
+          match fst (snd x) with
+          | Rle _ => match fst (snd y) with
+                     | Rle _ => False
+                     | Meth _ => True
+                     end
+          | Meth _ => True
+          end) /\
+      (forall x : MethT, InCall x (ModuleFilterLabels m1 l) -> InCall x (ModuleFilterLabels m2 l)
+                         -> False).
+  Proof.
+    induction 1; intros; split; auto; subst.
+    - intros; contradiction.
+    - unfold InCall; intros; dest; contradiction.
+    - simpl in HInRules.
+      destruct (in_app_or _ _ _ HInRules) as [Rle_in | Rle_in]; specialize (in_map fst _ _ Rle_in) as map_Rle_in; destruct (DisjRules rn); try contradiction;
+        intros x y; rewrite HLabel,(InRules_Filter u _ _ ls cs _ Rle_in);rewrite (NotInRules_Filter u _ ls cs _ H0); intros.
+        * destruct H1.
+          -- rewrite <- H1; simpl.
+             apply HNoRle.
+             unfold ModuleFilterLabels in H2; apply filter_In in H2; destruct H2; assumption.
+          -- eapply IHPSubsteps; eauto.
+        * destruct H2.
+          -- rewrite <- H2; simpl.
+             apply HNoRle.
+             unfold ModuleFilterLabels in H1; apply filter_In in H1; destruct H1; assumption.
+          -- eapply IHPSubsteps; eauto.
+    - destruct (in_app_or _ _ _ HInRules) as [Rle_in | Rle_in]; specialize (in_map fst _ _ Rle_in) as map_Rle_in; destruct (DisjRules rn); try contradiction;
+        intros x; rewrite HLabel,(InRules_Filter u _ _ ls cs _ Rle_in);rewrite (NotInRules_Filter u _ ls cs _ H0); intros.
+      + destruct (InCall_app_iff x (((u, (Rle rn, cs)))::nil) (ModuleFilterLabels m1 ls)) as [L R]; clear R.
+        destruct (L H1); clear L.
+        * unfold InCall in H3. dest.
+          destruct H3;[subst|contradiction].
+          apply InCall_split_InCall in H2.
+          apply (HNoCall x); auto.
+        * eapply IHPSubsteps; eauto.
+      + destruct (InCall_app_iff x (((u, (Rle rn, cs)))::nil) (ModuleFilterLabels m2 ls)) as [L R]; clear R.
+        destruct (L H2); clear L.
+        * unfold InCall in H3. dest.
+          destruct H3;[subst|contradiction].
+          apply InCall_split_InCall in H1.
+          apply (HNoCall x); auto.
+        * eapply IHPSubsteps; eauto.
+    - intros.
+      unfold ModuleFilterLabels in *.
+      rewrite HLabel in *.
+      specialize (filter_app (BaseModuleFilter m1) ((u, (Meth (fn, existT SignT (projT1 fb) (argV, retV)), cs))::nil) ls) as TMP; setoid_rewrite TMP in H0; clear TMP.
+      specialize (filter_app (BaseModuleFilter m2) ((u, (Meth (fn, existT SignT (projT1 fb) (argV, retV)), cs))::nil) ls) as TMP; setoid_rewrite TMP in H1; clear TMP.
+      destruct (in_app_or _ _ _ H0); destruct (in_app_or _ _ _ H1).
+      + apply filter_In in H3; apply filter_In in H2. dest.
+        destruct H2, H3; try contradiction.
+        subst; simpl; auto.
+      + apply filter_In in H2; destruct H2.
+        destruct H2;[|contradiction].
+        subst; simpl; auto.
+      + apply filter_In in H3; destruct H3.
+        destruct H3;[|contradiction].
+        subst; simpl; auto.
+        destruct (fst (snd x)); auto.
+      + eapply IHPSubsteps; eauto.
+    - intros.
+      destruct (DisjMeths fn).
+      + rewrite HLabel in *; setoid_rewrite (NotInMethods_Filter u _ fb argV retV ls cs _ H2) in H0.
+        unfold ModuleFilterLabels in *.
+        specialize (filter_app (BaseModuleFilter m2) ((u, (Meth (fn, existT SignT (projT1 fb) (argV, retV)), cs))::nil) ls) as TMP; setoid_rewrite TMP in H1; clear TMP.
+        destruct (InCall_app_iff x (filter (BaseModuleFilter m2) [(u, (Meth (fn, existT SignT (projT1 fb) (argV, retV)), cs))]) (filter (BaseModuleFilter m2) ls)) as [L R]; clear R; destruct (L H1); clear L.
+        * unfold InCall in H3; dest; apply filter_In in H3; destruct H3.
+          destruct H3;[subst|contradiction].
+          simpl in H6.
+          apply InCall_split_InCall in H0.
+          eapply HNoCall; eauto.
+        * eapply IHPSubsteps; eauto.
+      + rewrite HLabel in *; setoid_rewrite (NotInMethods_Filter u _ fb argV retV ls cs _ H2) in H1.
+        unfold ModuleFilterLabels in *.
+        specialize (filter_app (BaseModuleFilter m1) ((u, (Meth (fn, existT SignT (projT1 fb) (argV, retV)), cs))::nil) ls) as TMP; setoid_rewrite TMP in H0; clear TMP.
+        destruct (InCall_app_iff x (filter (BaseModuleFilter m1) [(u, (Meth (fn, existT SignT (projT1 fb) (argV, retV)), cs))]) (filter (BaseModuleFilter m1) ls)) as [L R]; clear R; destruct (L H0); clear L.
+        * unfold InCall in H3; dest; apply filter_In in H3; destruct H3.
+          destruct H3;[subst|contradiction].
+          simpl in H6.
+          apply InCall_split_InCall in H1.
+          eapply HNoCall; eauto.
+        * eapply IHPSubsteps; eauto.
+  Qed.
+
+End SplitSubsteps.
+
+Lemma PSubsteps_flatten m o l:
+  PSubsteps (BaseMod (getRegisters m) (getRules m) (getMethods m)) o l ->
+  PSubsteps m o l.
+Proof.
+  induction 1; simpl; auto.
+  - constructor 1; auto.
+  - econstructor 2; eauto.
+  - econstructor 3; eauto.
+Qed.
+
+Lemma flatten_PSubsteps m o l:
+  PSubsteps m o l ->
+  PSubsteps (BaseMod (getRegisters m) (getRules m) (getMethods m)) o l.
+  induction 1; simpl; auto.
+  - constructor 1; auto.
+  - econstructor 2; eauto.
+  - econstructor 3; eauto.
+Qed.
+
+Lemma PWfConcats m1 m2 o l:
+  WfConcat m2 m1 -> PSubsteps (getFlat m2) o l ->
+  forall s v,
+    In s (getHidden m1) -> ~InCall (s, v) l.
+Proof.
+  intros.
+  specialize (PSubsteps_Substeps H0) as TMP; dest.
+  specialize (WfConcats H H5 H1 (v:=v)).
+  repeat intro.
+  apply H6.
+  apply (List_FullLabel_perm_InCall_rewrite H3); assumption.
+Qed.
+
+Lemma substitute_PStep' m (HWfMod: WfMod m):
+  forall o l,
+    PStepSubstitute m o l ->
+    PStep m o l.
+Proof.
+  unfold PStepSubstitute.
+  induction m; simpl in *; intros; dest.
+  - constructor 1; auto; eapply PSubsteps_flatten; eauto.
+  - constructor; auto.
+    inv HWfMod;eapply IHm; eauto.
+  - inv HWfMod.
+    specialize (IHm1 HWf1).
+    specialize (IHm2 HWf2).
+    destruct (WfNoDups HWf1) as [ND_Regs1 [ND_Meths1 ND_Rules1]].
+    destruct (WfNoDups HWf2) as [ND_Regs2 [ND_Meths2 ND_Rules2]].
+    specialize (WfMod_WfBaseMod_flat HWf1) as WfBaseMod1.
+    specialize (WfMod_WfBaseMod_flat HWf2) as WfBaseMod2.
+    pose proof (@split_PSubsteps1 (getFlat m1) (getFlat m2) HDisjRegs HDisjRules HDisjMeths WfBaseMod1 WfBaseMod2 _ _  ND_Regs1 ND_Regs2 H);dest.
+    rewrite H4 in *.
+    assert (DisjKey (getRules (getFlat m1)) (getRules (getFlat m2)));[repeat intro; apply HDisjRules|].
+    assert (DisjKey (getMethods (getFlat m1))(getMethods (getFlat m2)));[repeat intro;apply HDisjMeths|].
+    specialize (pfilter_perm H7 H8 H) as P1.
+    rewrite P1. rewrite P1 in H.
+    econstructor 3.
+    + eapply IHm1; eauto.
+      Opaque MatchingExecCalls.
+      repeat split; eauto.
+      * unfold getFlat in H0; simpl in *.
+        assert (MatchingExecCalls l l (Base (concatFlat (getFlat m1) (getFlat m2))));[unfold concatFlat, getFlat;simpl; assumption|].
+        eapply MatchingExecCalls_Split; eauto.
+      * intros; specialize (H1 s v).
+        intros; specialize (PWfConcats WfConcat2 H6 H10 (v:=v));intro.
+        rewrite map_app in H1.
+        specialize (H1 (in_or_app _ _ s (or_introl H9)) (in_or_app _ _ s (or_introl H10)) (InExec_split_InExec _ _ _ H11)).
+        assert (DisjKey (getRules (getFlat m1)) (getRules (getFlat m2)));[repeat intro; apply HDisjRules|].
+        assert (DisjKey (getMethods (getFlat m1))(getMethods (getFlat m2)));[repeat intro;apply HDisjMeths|].
+        rewrite P1 in H1; apply InCall_app_iff in H1; destruct H1;[assumption|contradiction].
+    + eapply IHm2; eauto.
+      repeat split; eauto.
+      * unfold getFlat in H0; simpl in *.
+        assert (MatchingExecCalls l l (Base (concatFlat (getFlat m1) (getFlat m2))));[unfold concatFlat, getFlat;simpl; assumption|].
+        apply MatchingExecCalls_Concat_comm in H9.
+        eapply MatchingExecCalls_Split; eauto.
+      * intros; specialize (H1 s v).
+        intros; specialize (PWfConcats WfConcat1 H5 H10 (v:=v));intro.
+        rewrite map_app in H1.
+        specialize (H1 (in_or_app _ _ s (or_intror H9)) (in_or_app _ _ s (or_intror H10)) (InExec_split_InExec _ _ _ H11)).
+        assert (DisjKey (getRules (getFlat m1)) (getRules (getFlat m2)));[repeat intro; apply HDisjRules|].
+        assert (DisjKey (getMethods (getFlat m1))(getMethods (getFlat m2)));[repeat intro;apply HDisjMeths|].
+        rewrite P1 in H1; apply InCall_app_iff in H1; destruct H1;[contradiction|assumption].
+    + assert (MatchingExecCalls l l (Base (concatFlat (getFlat m1) (getFlat m2)))); auto.
+      specialize (MatchingExecCalls_Mix H9); intros.
+      Transparent MatchingExecCalls.
+      repeat intro.
+      destruct (H10 f H11 H12).
+      split; auto.
+      intro; apply (PWfConcats WfConcat1 H5 H15 (v:=(snd f))); destruct f ;assumption.
+    + assert (MatchingExecCalls l l (Base (concatFlat (getFlat m1) (getFlat m2)))); auto.
+      specialize (MatchingExecCalls_Mix (MatchingExecCalls_Concat_comm H9)); intros.
+      repeat intro.
+      destruct (H10 f H11 H12).
+      split; auto.
+      intro; apply (PWfConcats WfConcat2 H6 H15 (v:=(snd f))); destruct f ;assumption.
+    + intros.
+      eapply split_Substeps2; eauto; rewrite <- P1; assumption.
+    + eapply split_Substeps2; eauto; rewrite P1; apply H.
+    + reflexivity.
+    + reflexivity.
+Qed.
+
+
+Lemma substitute_PStep m o l (HWfMod: WfMod m):
+  PStep (flatten m) o l ->
+  PStep m o l.
+Proof.
+  rewrite PStepSubstitute_flatten in *; auto.
+  apply substitute_PStep'; auto.
+Qed.
+
+Section PTraceSubstitute.
+  Variable m: Mod.
+  Variable WfMod_m: WfMod m.
+
+  Lemma PTrace_flatten_same1: forall o l,  PTrace m o l -> PTrace (flatten m) o l.
+  Proof.
+    induction 1; subst.
+    - (constructor 1 with (o'':= o'')); unfold flatten; auto.
+      rewrite createHide_Regs.
+      auto.
+    - apply PStep_substitute in HPStep; auto.
+      econstructor 2; eauto.
+  Qed.
+
+  Lemma PTrace_flatten_same2: forall o l, PTrace (flatten m) o l -> PTrace m o l.
+  Proof.
+    induction 1; subst.
+    - rewrite getAllRegisters_flatten in *;constructor 1 with (o'' := o''); auto.
+    - apply substitute_PStep in HPStep;auto; dest.
+      + econstructor 2; eauto.
+  Qed.
+
+  Lemma PTraceInclusion_flatten_r: PTraceInclusion m (flatten m).
+  Proof.
+    unfold PTraceInclusion; intros.
+    exists ls.
+    split;[|apply WeakInclusionsRefl].
+    unfold PTraceList.
+    exists o.
+    apply PTrace_flatten_same1; assumption.
+  Qed.
+
+  Corollary TraceInclusion_flatten_r' : TraceInclusion m (flatten m).
+  Proof.
+    apply PTraceInclusion_TraceInclusion; eauto using flatten_WfMod.
+    apply PTraceInclusion_flatten_r.
+  Qed.
+  
+  Lemma PTraceInclusion_flatten_l: PTraceInclusion (flatten m) m.
+  Proof.
+    unfold PTraceInclusion; intros.
+    apply PTrace_flatten_same2 in H.
+    exists ls.
+    split.
+    - unfold PTraceList; exists o; auto.
+    - apply WeakInclusionsRefl.
+  Qed.
+
+  Corollary TraceInclusion_flatten_l' : TraceInclusion (flatten m) m.
+  Proof.
+    apply PTraceInclusion_TraceInclusion; eauto using flatten_WfMod.
+    apply PTraceInclusion_flatten_l.
+  Qed.
+  
+End PTraceSubstitute.
+
+
+Record WfModule : Type := mkWfMod {module :> Mod; Wf_cond : WfMod module}.
+
+Section WfModule_rewrite.
+
+  Inductive WfModule_perm : WfModule ->WfModule -> Prop :=
+  |Wf_perm_equiv (m m': WfModule) (HAllRegsPerm : getAllRegisters m [=] getAllRegisters m')
+              (HAllMethsPerm : getAllMethods m [=] getAllMethods m')
+              (HAllRulesPerm : getAllRules m [=] getAllRules m')
+              (HHiddenPerm : getHidden m [=] getHidden m') :
+     WfModule_perm m m'.
+
+  Lemma WfModule_perm_refl m :
+    WfModule_perm m m.
+  Proof.
+    constructor; auto.
+  Qed.
+
+  Lemma WfModule_perm_sym m m':
+    WfModule_perm m m' -> WfModule_perm m' m.
+  Proof.
+    constructor; inv H; eauto using Permutation_sym.
+  Qed.
+
+  Lemma WfModule_perm_trans m m' m'' :
+    WfModule_perm m m' -> WfModule_perm m' m'' -> WfModule_perm m m''.
+  Proof.
+    constructor; inv H; inv H0; eauto using Permutation_trans.
+  Qed.
+
+  Global Instance WfModule_perm_Equivalence : Equivalence (@WfModule_perm) | 10 := {
+     Equivalence_Reflexive := @WfModule_perm_refl;
+     Equivalence_Symmetric := @WfModule_perm_sym;             
+     Equivalence_Transitive:= @WfModule_perm_trans}.
+
+  
+  Lemma PStep_rewrite_base m1' m2' o l hl:
+    BaseModule_perm m1' m2' ->
+    PStep (createHide m1' hl) o l->
+    PStep (createHide m2' hl) o l.
+  Proof.
+    induction hl; simpl.
+    - intros.
+      inv H0; econstructor 1.
+      + rewrite <- H; assumption.
+      + repeat intro.
+        apply (HMatching f H0); simpl in *.
+        inversion H; subst.
+        rewrite HMethsPerm; assumption.
+    - intros.
+      inv H0; econstructor 2; auto; intros.
+      eapply HHidden; auto.
+      rewrite createHide_Meths in *.
+      inversion H; subst.
+      rewrite HMethsPerm; assumption.
+  Qed.
+
+Lemma PStep_rewrite_hides m o l:
+  forall hl' hl,
+    hl [=] hl' ->
+    PStep (createHide m hl) o l->
+    PStep (createHide m hl') o l.
+Proof.
+  induction 1; auto; intros.
+  - simpl in *; inv H0; econstructor 2;  auto.
+    intros.
+    rewrite createHide_Meths in *.
+    eapply HHidden; eauto.
+  - simpl in *.
+    inv H; inv HPStep.
+    econstructor 2;[econstructor 2|]; auto.
+Qed.
+  
+  Lemma PStep_WfModule_rewrite m1 m2 o l :
+    WfModule_perm m1 m2 ->
+    PStep m1 o l ->
+    PStep m2 o l.
+  Proof.
+    intros.
+    apply (substitute_PStep); eauto using (Wf_cond m2).
+    apply (PStep_substitute) in H0; eauto using (Wf_cond m1).
+    unfold flatten in *.
+    assert (BaseModule_perm (getFlat m1) (getFlat m2));[inv H;unfold getFlat;constructor;auto|].
+    apply (PStep_rewrite_base (getHidden m1) H1) in H0.
+    inv H.
+    apply (PStep_rewrite_hides _ HHiddenPerm H0).
+  Qed.
+
+  Lemma Forall2_perm (A B : Type) (* (l1 : list A) *)
+        (l2 l3 : list B)(P : A -> B -> Prop):
+    l2 [=] l3 ->
+    forall l1,
+    Forall2 P l1 l2 ->
+    (exists l4,
+        l1 [=] l4 /\
+        Forall2 P l4 l3).
+    induction 1.
+    - intros; inv H.
+      exists nil; split; eauto.
+    - intros.
+      destruct l1; inv H0.
+      specialize (IHPermutation _ H6);dest.
+      exists (a::x0).
+      split; auto.
+    - intros.
+      destruct l1; inv H.
+      destruct l1; inv H5.
+      exists (a0::a::l1); split; auto.
+      econstructor 3.
+    - intros.
+      specialize (IHPermutation1 _ H1);dest.
+      specialize (IHPermutation2 _ H3);dest.
+      exists x0; split; eauto using Permutation_trans.
+  Qed.
+  
+  Lemma PTrace_WfModule_rewrite m1 m2 o ls:
+    WfModule_perm m1 m2 ->
+    PTrace m1 o ls ->
+    PTrace m2 o ls.
+  Proof.
+    induction 2; subst; inv H.
+    - specialize (Forall2_perm  HAllRegsPerm HUpdRegs) as TMP; dest.
+      econstructor 1 with (o'':=x);eauto.
+      rewrite <- H; assumption.
+    - econstructor 2; eauto.
+      eapply (PStep_WfModule_rewrite) in HPStep; eauto.
+      econstructor; eauto.
+  Qed.
+
+  Lemma PTrace_RegsT_rewrite m o1 o2 ls :
+    o1 [=] o2 ->
+    PTrace m o1 ls ->
+    PTrace m o2 ls.
+  Proof.
+    intros; inv H0.
+    - econstructor 1 with (o'':=o''); eauto using Permutation_sym, Permutation_trans.
+    - econstructor 2; eauto.
+      unfold PUpdRegs in *; dest.
+      repeat split; auto.
+      + rewrite <- H; assumption.
+      + intros.
+        rewrite <- H in H2.
+        specialize (H1 s v H2).
+        assumption.
+  Qed.
+
+  Lemma PTrace_rewrite m1 m2 o1 o2 ls:
+    o1 [=] o2 ->
+    WfModule_perm m1 m2 ->
+    PTrace m1 o1 ls ->
+    PTrace m2 o2 ls.
+  Proof.
+    intros; eauto using PTrace_WfModule_rewrite, PTrace_RegsT_rewrite.
+  Qed.
+
+  Global Instance PStep_WfModule_rewrite' :
+    Proper (@WfModule_perm ==> Logic.eq ==> Logic.eq ==> iff) (@PStep) |10.
+  Proof.
+    repeat red; split; intros; subst; eauto using WfModule_perm_sym,PStep_WfModule_rewrite.
+  Qed.
+
+  Global Instance Trace_rewrite' :
+    Proper (@WfModule_perm ==> @Permutation (string * {x : FullKind & fullType type x}) ==> Logic.eq ==> iff) (@PTrace) | 10.
+  Proof.
+    repeat red; split; intros; subst; eauto using WfModule_perm_sym, Permutation_sym, PTrace_rewrite.
+  Qed.
+End WfModule_rewrite.
+
+Lemma WfNilMod :
+  WfMod (Base (BaseMod nil nil nil)).
+Proof.
+  constructor; simpl; constructor; intros; contradiction.
+Qed.
+
+Lemma WfConcatActionTNil (k : Kind) (a : ActionT type k):
+  WfConcatActionT a (Base (BaseMod nil nil nil)).
+Proof.
+  induction a; econstructor; eauto.
+Qed.
+
+Lemma WfConcatNil m :
+  WfMod m ->
+  WfMod (ConcatMod m (Base (BaseMod nil nil nil))).
+Proof.
+  constructor; unfold DisjKey; simpl; intros; auto.
+  - apply WfNilMod.
+  - split; intros; eauto using WfConcatActionTNil.
+  - split; intros; contradiction.
+Qed.
+
+Lemma WfNilConcat m :
+  WfMod (ConcatMod m (Base (BaseMod nil nil nil))) ->
+  WfMod m.
+Proof.
+  intros; inv H; assumption.
+Qed.
+
+Lemma WfConcatComm m1 m2 :
+  WfMod (ConcatMod m1 m2) ->
+  WfMod (ConcatMod m2 m1).
+Proof.
+  intros; inv H.
+  econstructor; eauto using DisjKey_Commutative.
+Qed.
+
+Lemma DeM1 (A : Type):
+  forall (l1 l2 : list A) (a : A),
+    ~(In a l1 \/ In a l2) <-> ~In a l1 /\ ~In a l2.
+Proof.
+  split;intros.
+  - split; intro; apply H; auto.
+  - destruct H.
+    intro; destruct H1; auto.
+Qed.
+
+Lemma WfConcatSplits m1 m2 (k : Kind) (a : ActionT type k):
+    WfConcatActionT a (ConcatMod m1 m2) ->
+    WfConcatActionT a m1 /\
+    WfConcatActionT a m2.
+Proof.
+  induction a.
+  - intros; split; econstructor 1; eauto; inv H0; EqDep_subst; intro; try eapply H; eauto;
+      apply H8; simpl; rewrite in_app_iff; eauto.
+  - intros; split; econstructor 2; eauto; inv H0; EqDep_subst; destruct (H (evalExpr e) H6); auto.
+  - intros; split; econstructor 3; eauto; inv H0; EqDep_subst; try intro; try eapply IHa; eauto;
+    eapply H; eauto.
+  - intros; split; econstructor 4; eauto; inv H0; EqDep_subst; intros; eapply H; eauto.
+  - intros; split; econstructor 5; eauto; inv H0; EqDep_subst; intros; eapply H; eauto.
+  - intros; split; econstructor 6; eauto; inv H; EqDep_subst; eapply IHa; eauto.
+  - intros; split; econstructor 7; eauto; inv H0; EqDep_subst; try intros; try eapply H; eauto;
+      try eapply IHa1; eauto; eapply IHa2; eauto.
+  - intros; split; econstructor 8; eauto; inv H; EqDep_subst; eapply IHa; eauto.
+  - intros; split; econstructor 9; eauto; inv H; EqDep_subst; eapply IHa; eauto.
+  - intros; split; econstructor 10.
+Qed.
+
+Lemma WfConcatMerge m1 m2 (k : Kind) (a : ActionT type k) :
+  WfConcatActionT a m1 ->
+  WfConcatActionT a m2 ->
+  WfConcatActionT a (ConcatMod m1 m2).
+Proof.
+  induction a; intros.
+  - econstructor 1; inv H0; inv H1; EqDep_subst; intros; try eapply H; eauto; simpl; rewrite in_app_iff; intro;
+      destruct H0;auto.
+  - econstructor 2; inv H0; inv H1; EqDep_subst; eapply H; eauto.
+  - econstructor 3; inv H0; inv H1; EqDep_subst; try eapply H; eauto.
+  - econstructor 4; inv H0; inv H1; EqDep_subst; intros; eapply H; eauto.
+  - econstructor 5; inv H0; inv H1; EqDep_subst; intros; eapply H; eauto.
+  - econstructor 6; inv H; inv H0; EqDep_subst; eapply IHa; eauto.
+  - econstructor 7; inv H0; inv H1; EqDep_subst; intros; try eapply H, IHa1, IHa2; eauto.
+  - econstructor 8; inv H; inv H0; EqDep_subst; eapply IHa; eauto.
+  - econstructor 9; inv H; inv H0; EqDep_subst; eapply IHa; eauto.
+  - econstructor 10.
+Qed.
+    
+
+Lemma WfConcatAssoc1 m1 m2 m3 :
+  WfMod (ConcatMod m1 (ConcatMod m2 m3)) ->
+  WfMod (ConcatMod (ConcatMod m1 m2) m3).
+Proof.
+  intros; inv H; inv HWf2; inv WfConcat1; inv WfConcat2.
+  econstructor; simpl in *; eauto.
+  - intro.
+    destruct (HDisjRegs k), (HDisjRegs0 k); simpl in *; rewrite map_app in *; rewrite in_app_iff in *; rewrite DeM1 in *; auto.
+    destruct H3; right; assumption.
+  - intro.
+    destruct (HDisjRules k), (HDisjRules0 k); simpl in *; rewrite map_app in *; rewrite in_app_iff in *; rewrite DeM1 in *; auto.
+    destruct H3; right; assumption.
+  - intro.
+    destruct (HDisjMeths k), (HDisjMeths0 k); simpl in *; rewrite map_app in *; rewrite in_app_iff in *; rewrite DeM1 in *; auto.
+    destruct H3; right; assumption.
+  - econstructor; eauto; simpl in *.
+    + intro.
+      destruct (HDisjRegs k), (HDisjRegs0 k); simpl in *; auto; rewrite map_app in *; rewrite in_app_iff in *; rewrite DeM1 in *; auto.
+      destruct H3; right; assumption.
+    + intro.
+      destruct (HDisjRules k), (HDisjRules0 k); simpl in *; auto; rewrite map_app in *; rewrite in_app_iff in *; rewrite DeM1 in *.
+      destruct H3; right; assumption.
+    + intro.
+      destruct (HDisjMeths k), (HDisjMeths0 k); simpl in *; auto; rewrite map_app in *; rewrite in_app_iff in *; rewrite DeM1 in *.
+      destruct H3; right; assumption.
+    + econstructor; intros.
+      * specialize (H _ H3).
+        apply (WfConcatSplits H).
+      * specialize (H0 _ H3 v).
+        apply (WfConcatSplits H0).
+    + econstructor; intros.
+      * apply (H1 rule (in_or_app _ _ _ (or_introl _ H3))).
+      * apply (H2 meth (in_or_app _ _ _ (or_introl _ H3)) v).
+  - split; intros; simpl in *; rewrite in_app_iff in *; destruct H3.
+    + specialize (H _ H3); apply (WfConcatSplits H).
+    + inv WfConcat0; eauto.
+    + specialize (H0 _ H3 v); apply (WfConcatSplits H0).
+    + inv WfConcat0; eauto.
+  - split; intros; simpl in *;inv WfConcat3.
+    + eapply WfConcatMerge; eauto.
+      apply (H1 rule (in_or_app _ _ _ (or_intror _ H3))).
+    + eapply WfConcatMerge; eauto.
+      apply (H2 meth (in_or_app _ _ _ (or_intror _ H3)) v).
+Qed.
+
+
+Lemma WfConcatAssoc2 m1 m2 m3 :
+  WfMod (ConcatMod (ConcatMod m1 m2) m3) ->
+  WfMod (ConcatMod m1 (ConcatMod m2 m3)).
+Proof.
+  intros.
+  inv H; inv HWf1; inv WfConcat1; inv WfConcat2.
+  econstructor; try intro; simpl in *; eauto.
+  - destruct (HDisjRegs k), (HDisjRegs0 k); simpl in *; rewrite map_app in *; rewrite in_app_iff in *; rewrite DeM1 in *; auto.
+    destruct H3; left; assumption.
+  - destruct (HDisjRules k), (HDisjRules0 k); simpl in *; rewrite map_app in *; rewrite in_app_iff in *; rewrite DeM1 in *; auto.
+    destruct H3; left; assumption.
+  - destruct (HDisjMeths k), (HDisjMeths0 k); simpl in *; rewrite map_app in *; rewrite in_app_iff in *; rewrite DeM1 in *; auto.
+    destruct H3; left; assumption.
+  - econstructor; try intro; simpl in *; eauto.
+    + destruct (HDisjRegs k), (HDisjRegs0 k); simpl in *; auto; rewrite map_app in *; rewrite in_app_iff in *; rewrite DeM1 in *.
+      destruct H3; left; assumption.
+    + destruct (HDisjRules k), (HDisjRules0 k); simpl in *; auto; rewrite map_app in *; rewrite in_app_iff in *; rewrite DeM1 in *.
+      destruct H3; left; assumption.
+    + destruct (HDisjMeths k), (HDisjMeths0 k); simpl in *; auto; rewrite map_app in *; rewrite in_app_iff in *; rewrite DeM1 in *.
+      destruct H3; left; assumption.
+    + split; intros.
+      * apply (H rule (in_or_app _ _ _ (or_intror _ H3))).
+      * apply (H0 meth (in_or_app _ _ _ (or_intror _ H3)) v).
+    + split; intros.
+      * eapply WfConcatSplits; eauto.
+      * eapply WfConcatSplits; eauto.
+  -  split; intros; inv WfConcat0; inv WfConcat3.
+     + eapply WfConcatMerge; eauto.
+       apply (H rule (in_or_app _ _ _ (or_introl _ H3))).
+     + eapply WfConcatMerge; eauto.
+       apply (H0 meth (in_or_app _ _ _ (or_introl _ H3)) v).
+  - econstructor; intros; simpl in *; rewrite in_app_iff in *; destruct H3; inv WfConcat0; inv WfConcat3;
+      eauto; eapply (WfConcatSplits (m1 :=m1) (m2 := m2)); eauto.
+Qed.
+
+Lemma WfMod_createHide' l : forall m, WfMod (createHide' m l) <-> (SubList l (map fst (getAllMethods m)) /\ WfMod m).
+Proof.
+  split.
+  - induction l; simpl; intros; split; auto.
+    + repeat intro; contradiction.
+    + inv H.
+      specialize (IHl HWf); dest.
+      repeat intro.
+      destruct H1; subst; rewrite getAllMethods_createHide' in HHideWf; auto.
+    + inv H.
+      specialize (IHl HWf); dest; auto.
+  - induction l; intros; dest; simpl; eauto.
+    destruct (SubList_cons H).
+    econstructor; eauto.
+    rewrite getAllMethods_createHide'; auto.
+Qed.
+
+Lemma SeparatedBaseMod_concat l1 l2:
+  getAllRegisters (mergeSeparatedBaseMod (l1++l2)) [=] getAllRegisters (mergeSeparatedBaseMod l1) ++ getAllRegisters (mergeSeparatedBaseMod l2).
+Proof.
+  induction l1.
+  - simpl; reflexivity.
+  - simpl.
+    rewrite <- app_assoc.
+    apply Permutation_app_head.
+    rewrite IHl1.
+    reflexivity.
+Qed.
+
+Lemma SeparatedBaseMod_concat_Rules l1 l2:
+  getAllRules (mergeSeparatedBaseMod (l1++l2)) [=] getAllRules (mergeSeparatedBaseMod l1) ++ getAllRules (mergeSeparatedBaseMod l2).
+Proof.
+  induction l1.
+  - simpl; reflexivity.
+  - simpl.
+    rewrite <- app_assoc.
+    apply Permutation_app_head.
+    rewrite IHl1.
+    reflexivity.
+Qed.
+
+Lemma SeparatedBaseMod_concat_Meths l1 l2:
+  getAllMethods (mergeSeparatedBaseMod (l1++l2)) [=] getAllMethods (mergeSeparatedBaseMod l1) ++ getAllMethods (mergeSeparatedBaseMod l2).
+Proof.
+  induction l1.
+  - simpl; reflexivity.
+  - simpl.
+    rewrite <- app_assoc.
+    apply Permutation_app_head.
+    rewrite IHl1.
+    reflexivity.
+Qed.
+
+Lemma SeparatedBaseFile_concat l1 l2:
+  getAllRegisters (mergeSeparatedBaseFile (l1++l2)) [=] getAllRegisters (mergeSeparatedBaseFile l1) ++ getAllRegisters (mergeSeparatedBaseFile l2).
+Proof.
+  induction l1.
+  - simpl; reflexivity.
+  - simpl.
+    rewrite <- app_assoc.
+    apply Permutation_app_head.
+    rewrite IHl1.
+    reflexivity.
+Qed.
+
+Lemma SeparatedBaseFile_concat_Rules l1 l2:
+  getAllRules (mergeSeparatedBaseFile (l1++l2)) [=] getAllRules (mergeSeparatedBaseFile l1) ++ getAllRules (mergeSeparatedBaseFile l2).
+Proof.
+  induction l1.
+  - simpl; reflexivity.
+  - simpl; assumption.
+Qed.
+
+Lemma SeparatedBaseFile_concat_Meths l1 l2:
+  getAllMethods (mergeSeparatedBaseFile (l1++l2)) [=] getAllMethods (mergeSeparatedBaseFile l1) ++ getAllMethods (mergeSeparatedBaseFile l2).
+Proof.
+  induction l1.
+  - simpl; reflexivity.
+  - simpl.
+    rewrite <- app_assoc.
+    apply Permutation_app_head.
+    rewrite IHl1.
+    reflexivity.
+Qed.
+
+Lemma DisjKey_perm_rewrite (A B : Type) (l1 l2 l3 l4 : list (A*B)) :
+  l1 [=] l2 ->
+  l3 [=] l4 ->
+  DisjKey l1 l3 ->
+  DisjKey l2 l4.
+Proof.
+  repeat intro; destruct (H1 k); [left; rewrite <- H|right; rewrite <- H0]; auto.
+Qed.
+
+Global Instance DisjKey_perm_rewrite' A B :
+  Proper (@Permutation (A*B) ==> @Permutation (A*B) ==> iff) (@DisjKey A B) | 10.
+Proof.
+  repeat red; intros; split; intros; eauto using DisjKey_perm_rewrite, Permutation_sym.
+Qed.
+
+Lemma WfActionTConcatAssoc1 m1 m2 m3 (k : Kind) (a : ActionT type k) :
+  WfConcatActionT a (ConcatMod (ConcatMod m1 m2) m3) ->
+  WfConcatActionT a (ConcatMod m1 (ConcatMod m2 m3)).
+Proof.
+  intros.
+  induction a; inv H; econstructor; EqDep_subst; intros; simpl in *; eauto.
+    rewrite app_assoc; assumption.
+Qed.
+
+
+Lemma WfActionTConcatAssoc2 m1 m2 m3 (k : Kind) (a : ActionT type k) :
+  WfConcatActionT a (ConcatMod m1 (ConcatMod m2 m3)) ->
+  WfConcatActionT a (ConcatMod (ConcatMod m1 m2) m3).
+Proof.
+  intros.
+  induction a; inv H; econstructor; EqDep_subst; intros; simpl in *; eauto.
+    rewrite <- app_assoc; assumption.
+Qed.
+
+Lemma WfConcatBaseFiles l1 l2 (k : Kind) (a : ActionT type k):
+  WfConcatActionT a (ConcatMod (mergeSeparatedBaseFile l1) (mergeSeparatedBaseFile l2)) ->
+  WfConcatActionT a (mergeSeparatedBaseFile (l1 ++ l2)).
+Proof.
+  induction l1.
+  - intros.
+    apply WfConcatSplits in H; dest; assumption.
+  - simpl.
+    intros.
+    apply WfActionTConcatAssoc1  in H.
+    apply WfConcatSplits in H; dest.
+    apply WfConcatMerge; eauto.
+Qed.
+
+Lemma WfConcatBaseModules l1 l2 (k : Kind) (a : ActionT type k):
+  WfConcatActionT a (ConcatMod (mergeSeparatedBaseMod l1) (mergeSeparatedBaseMod l2)) ->
+  WfConcatActionT a (mergeSeparatedBaseMod (l1 ++ l2)).
+Proof.
+  induction l1.
+  - intros.
+    apply WfConcatSplits in H; dest; assumption.
+  - simpl.
+    intros.
+    apply WfActionTConcatAssoc1  in H.
+    apply WfConcatSplits in H; dest.
+    apply WfConcatMerge; eauto.
+Qed.
+
+Lemma WfAppBaseFiles l1 l2:
+  WfMod (mergeSeparatedBaseFile l1) ->
+  WfMod (mergeSeparatedBaseFile l2) ->
+  WfMod (ConcatMod (mergeSeparatedBaseFile l1) (mergeSeparatedBaseFile l2)) ->
+  WfMod (mergeSeparatedBaseFile (l1 ++ l2)).
+Proof.
+  induction l1; intros; simpl in *; auto.
+  apply WfConcatAssoc2 in H1.
+  econstructor; inv H1; simpl in *; auto.
+  - rewrite <- SeparatedBaseFile_concat in HDisjRegs; assumption.
+  - intro; left; intro; contradiction.
+  - rewrite <- SeparatedBaseFile_concat_Meths in HDisjMeths; assumption.
+  - pose proof (HWf2) as HWf2'.
+    inv HWf2; eapply IHl1; eauto.
+  - split; intros; destruct WfConcat1.
+    + simpl in *; contradiction.
+    + specialize (H3 _ H1 v).
+      apply WfConcatBaseFiles in H3; assumption.
+  - split; intros; destruct WfConcat2.
+    rewrite getAllRules_mergeBaseFile in H1; contradiction.
+    simpl in H3; repeat rewrite getAllMethods_mergeBaseFile in *.
+    rewrite map_app, concat_app in *.
+    specialize (H3 _ H1 v); assumption.
+Qed.
+
+Lemma WfAppBaseMods l1 l2:
+  WfMod (mergeSeparatedBaseMod l1) ->
+  WfMod (mergeSeparatedBaseMod l2) ->
+  WfMod (ConcatMod (mergeSeparatedBaseMod l1) (mergeSeparatedBaseMod l2)) ->
+  WfMod (mergeSeparatedBaseMod (l1 ++ l2)).
+Proof.
+  induction l1; intros; simpl in *; auto.
+  apply WfConcatAssoc2 in H1.
+  econstructor; inv H1; simpl in *; auto.
+  - rewrite <- SeparatedBaseMod_concat in HDisjRegs; assumption.
+  - rewrite <- SeparatedBaseMod_concat_Rules in HDisjRules; assumption.
+  - rewrite <- SeparatedBaseMod_concat_Meths in HDisjMeths; assumption.
+  - pose proof (HWf2) as HWf2'.
+    inv HWf2; eapply IHl1; eauto.
+  - split; intros; destruct WfConcat1.
+    +  specialize (H2 _ H1).
+       apply WfConcatBaseModules in H2; assumption.
+    + specialize (H3 _ H1 v).
+      apply WfConcatBaseModules in H3; assumption.
+  - split; intros; destruct WfConcat2.
+    + simpl in *.
+      repeat rewrite getAllRules_mergeBaseMod in *.
+      rewrite map_app, concat_app in *.
+      specialize (H2 _ H1); assumption.
+    + simpl in H3; repeat rewrite getAllMethods_mergeBaseMod in *.
+      rewrite map_app, concat_app in *.
+      specialize (H3 _ H1 v); assumption.
+Qed.
+
+
+Lemma Base_File_Disjoint_Registers m :
+  WfMod m ->
+  DisjKey (getAllRegisters (mergeSeparatedBaseFile (fst (separateBaseMod m)))) (getAllRegisters (mergeSeparatedBaseMod (snd (separateBaseMod m)))).
+Proof.
+  intros; induction m; inv H.
+  - destruct m; simpl; rewrite app_nil_r; repeat intro;[right|left];intro; contradiction.
+  - specialize (IHm HWf).
+    simpl; assumption.
+  - specialize (IHm1 HWf1); specialize (IHm2 HWf2).
+    intro.
+    destruct (HDisjRegs k).
+    + rewrite separateBaseMod_flatten in H; simpl in H.
+      unfold mergeSeparatedMod in H.
+      rewrite getAllRegisters_createHide' in H; simpl in *; rewrite map_app,in_app_iff, DeM1 in H; dest.
+      destruct (separateBaseMod m1), (separateBaseMod m2); simpl.
+      rewrite SeparatedBaseMod_concat, SeparatedBaseFile_concat; repeat rewrite map_app, in_app_iff; repeat rewrite DeM1.
+      destruct (IHm1 k), (IHm2 k); simpl in *.
+      * left; split; auto.
+      * right; split; auto.
+      * left; split; auto.
+      * right; split; auto.
+    + rewrite separateBaseMod_flatten in H; simpl in H.
+      unfold mergeSeparatedMod in H.
+      rewrite getAllRegisters_createHide' in H; simpl in *; rewrite map_app,in_app_iff, DeM1 in H; dest.
+      destruct (separateBaseMod m1), (separateBaseMod m2); simpl.
+      rewrite SeparatedBaseMod_concat, SeparatedBaseFile_concat; repeat rewrite map_app, in_app_iff; repeat rewrite DeM1.
+      destruct (IHm1 k), (IHm2 k); simpl in *.
+      * left; split; auto.
+      * left; split; auto.
+      * right; split; auto.
+      * right; split; auto.
+Qed.
+
+Lemma WfActionBreakDownFile m (k : Kind) (a : ActionT type k): 
+  WfConcatActionT a m -> WfConcatActionT a (mergeSeparatedBaseFile (fst (snd (separateMod m)))).
+Proof.
+  induction a; simpl; intros; econstructor; intros; try inv H0; try inv H; EqDep_subst; eauto.
+  - rewrite mergeSeparatedBaseFile_noHides; intro; contradiction.
+Qed.
+
+Lemma WfActionBreakDownMod m (k : Kind) (a : ActionT type k): 
+  WfConcatActionT a m -> WfConcatActionT a (mergeSeparatedBaseMod (snd (snd (separateMod m)))).
+Proof.
+  induction a; simpl; intros; econstructor; intros; try inv H0; try inv H; EqDep_subst; eauto.
+  - rewrite mergeSeparatedBaseMod_noHides; intro; contradiction.
+Qed.
+
+Lemma WfModBreakDownFile m :
+  WfMod m ->
+  WfMod (mergeSeparatedBaseFile (fst (snd (separateMod m)))).
+Proof.
+  induction m.
+  - destruct m; simpl; intros; eauto using WfConcatNil, WfNilMod.
+  - intro; inv H; simpl; eapply IHm; eauto.
+  - intro; inv H.
+    rewrite (separateBaseMod_flatten m1), (separateBaseMod_flatten m2) in HDisjRegs.
+    rewrite (separateBaseModule_flatten_Rules m1), (separateBaseModule_flatten_Rules m2) in HDisjRules.
+    rewrite (separateBaseModule_flatten_Methods m1), (separateBaseModule_flatten_Methods m2) in HDisjMeths.
+    inv WfConcat1; inv WfConcat2.
+    setoid_rewrite (separateBaseModule_flatten_Rules m1) in H; setoid_rewrite  (separateBaseModule_flatten_Rules m2) in H1.
+    setoid_rewrite  (separateBaseModule_flatten_Methods m1) in H0; setoid_rewrite  (separateBaseModule_flatten_Methods m2) in H2.
+    simpl in *.
+    unfold mergeSeparatedMod in *; repeat rewrite getAllRegisters_createHide' in *; repeat rewrite getAllMethods_createHide' in *; repeat rewrite getAllRules_createHide' in *; simpl in *.
+    remember (separateBaseMod m1) as sbm1; remember (separateBaseMod m2) as sbm2.
+    destruct sbm1, sbm2; simpl in *.
+    apply WfAppBaseFiles; eauto.
+    econstructor; eauto.
+    + intro; specialize (HDisjRegs k); repeat rewrite map_app, in_app_iff, DeM1 in *.
+      destruct HDisjRegs; dest; eauto.
+    + intro; specialize (HDisjRules k); repeat rewrite map_app, in_app_iff, DeM1 in *.
+      destruct HDisjRules; dest; eauto.
+    + intro; specialize (HDisjMeths k); repeat rewrite map_app, in_app_iff, DeM1 in *.
+      destruct HDisjMeths; dest; eauto.
+    + split; intros.
+      * setoid_rewrite in_app_iff in H.
+        specialize (H _ (or_introl _ H3)).
+        apply WfActionBreakDownFile in H.
+        unfold separateMod in H; simpl in *; rewrite <- Heqsbm2 in H; simpl in *; assumption.
+      * setoid_rewrite in_app_iff in H0.
+        specialize (H0 _ (or_introl _ H3) v).
+        apply WfActionBreakDownFile in H0.
+        unfold separateMod in H0; simpl in *; rewrite <- Heqsbm2 in H0; simpl in *; assumption.
+    + split; intros.
+      * setoid_rewrite in_app_iff in H1.
+        specialize (H1 _ (or_introl _ H3)).
+        apply WfActionBreakDownFile in H1.
+        unfold separateMod in H1; simpl in *; rewrite <- Heqsbm1 in H1; simpl in *; assumption.
+      * setoid_rewrite in_app_iff in H2.
+        specialize (H2 _ (or_introl _ H3) v).
+        apply WfActionBreakDownFile in H2.
+        unfold separateMod in H2; simpl in *; rewrite <- Heqsbm1 in H2; simpl in *; assumption.
+Qed.
+
+Lemma WfModBreakDownMod m :
+  WfMod m ->
+  WfMod (mergeSeparatedBaseMod (snd (snd (separateMod m)))).
+Proof.
+  induction m.
+  - destruct m; simpl; intros; eauto using WfConcatNil, WfNilMod.
+  - intro; inv H; simpl; eapply IHm; eauto.
+  - intro; inv H.
+    rewrite (separateBaseMod_flatten m1), (separateBaseMod_flatten m2) in HDisjRegs.
+    rewrite (separateBaseModule_flatten_Rules m1), (separateBaseModule_flatten_Rules m2) in HDisjRules.
+    rewrite (separateBaseModule_flatten_Methods m1), (separateBaseModule_flatten_Methods m2) in HDisjMeths.
+    inv WfConcat1; inv WfConcat2.
+    setoid_rewrite (separateBaseModule_flatten_Rules m1) in H; setoid_rewrite  (separateBaseModule_flatten_Rules m2) in H1.
+    setoid_rewrite  (separateBaseModule_flatten_Methods m1) in H0; setoid_rewrite  (separateBaseModule_flatten_Methods m2) in H2.
+    simpl in *.
+    unfold mergeSeparatedMod in *; repeat rewrite getAllRegisters_createHide' in *; repeat rewrite getAllMethods_createHide' in *; repeat rewrite getAllRules_createHide' in *; simpl in *.
+    remember (separateBaseMod m1) as sbm1; remember (separateBaseMod m2) as sbm2.
+    destruct sbm1, sbm2; simpl in *.
+    apply WfAppBaseMods; eauto.
+    econstructor; eauto.
+    + intro; specialize (HDisjRegs k); repeat rewrite map_app, in_app_iff, DeM1 in *.
+      destruct HDisjRegs; dest; eauto.
+    + intro; specialize (HDisjRules k); repeat rewrite map_app, in_app_iff, DeM1 in *.
+      destruct HDisjRules; dest; eauto.
+    + intro; specialize (HDisjMeths k); repeat rewrite map_app, in_app_iff, DeM1 in *.
+      destruct HDisjMeths; dest; eauto.
+    + split; intros.
+      * setoid_rewrite in_app_iff in H.
+        specialize (H _ (or_intror _ H3)).
+        apply WfActionBreakDownMod in H.
+        unfold separateMod in H; simpl in *; rewrite <- Heqsbm2 in H; simpl in *; assumption.
+      * setoid_rewrite in_app_iff in H0.
+        specialize (H0 _ (or_intror _ H3) v).
+        apply WfActionBreakDownMod in H0.
+        unfold separateMod in H0; simpl in *; rewrite <- Heqsbm2 in H0; simpl in *; assumption.
+    + split; intros.
+      * setoid_rewrite in_app_iff in H1.
+        specialize (H1 _ (or_intror _ H3)).
+        apply WfActionBreakDownMod in H1.
+        unfold separateMod in H1; simpl in *; rewrite <- Heqsbm1 in H1; simpl in *; assumption.
+      * setoid_rewrite in_app_iff in H2.
+        specialize (H2 _ (or_intror _ H3) v).
+        apply WfActionBreakDownMod in H2.
+        unfold separateMod in H2; simpl in *; rewrite <- Heqsbm1 in H2; simpl in *; assumption.
+Qed.
+
+Lemma WfConcat_noHide m1 m2 :
+  getHidden m2 = nil ->
+  WfConcat m1 m2.
+Proof.
+  intros.
+  split; intros.
+  - induction (snd rule type); econstructor; eauto.
+    rewrite H; intro; contradiction.
+  - induction (projT2 (snd meth) type v); econstructor; eauto.
+    rewrite H; intro; contradiction.
+Qed.
+
+Lemma merged_WellFormed m:
+  WfMod m ->
+  WfMod (mergeSeparatedMod (fst (separateMod m)) (fst (snd (separateMod m))) (snd (snd (separateMod m)))).
+Proof.
+  induction 1.
+  - destruct m; simpl in *.
+    + unfold mergeSeparatedMod; simpl.
+      repeat apply WfConcatNil.
+      econstructor; eauto.
+    + unfold mergeSeparatedMod; simpl.
+      apply WfConcatAssoc2,WfConcatNil,WfConcatComm,WfConcatNil.
+      econstructor; eauto.
+  - unfold mergeSeparatedMod in *.
+    rewrite WfMod_createHide' in *; dest; simpl in *; split; eauto.
+    + unfold SubList; intros.
+      destruct H2; subst.
+      * rewrite (separateBaseModule_flatten_Methods m) in HHideWf.
+        unfold mergeSeparatedMod in HHideWf. rewrite getAllMethods_createHide' in HHideWf; simpl in *; assumption.
+      * eapply H0; eauto.
+  - unfold mergeSeparatedMod in *.
+    rewrite WfMod_createHide' in *; dest; split.
+    + unfold separateMod in *.
+      repeat intro.
+      specialize (separateBaseModule_flatten_Methods (ConcatMod m1 m2)) as TMP1.
+      specialize (separateBaseModule_flatten_Methods m1) as TMP2.
+      specialize (separateBaseModule_flatten_Methods m2) as TMP3.
+      unfold mergeSeparatedMod in *; rewrite getAllMethods_createHide' in *.
+      rewrite <- TMP1.
+      rewrite <- TMP2 in H3.
+      rewrite <- TMP3 in H1.
+      simpl in *; rewrite map_app in *; rewrite in_app_iff in *.
+      destruct H5.
+      * left; eapply H3; eauto.
+      * right; eapply H1; eauto.
+    + inv H4; inv H2.
+      econstructor.
+      * specialize (separateBaseMod_flatten (ConcatMod m1 m2)) as TMP1;
+        specialize (separateBaseMod_flatten m1) as TMP2; specialize (separateBaseMod_flatten m2) as TMP3.
+        unfold mergeSeparatedMod in *; rewrite getAllRegisters_createHide' in *; simpl in *; intro.
+        specialize (HDisjRegs k); rewrite TMP2, TMP3 in HDisjRegs.
+        repeat rewrite map_app,in_app_iff,DeM1 in *.
+        destruct (separateBaseMod m1), (separateBaseMod m2); simpl in *.
+        rewrite SeparatedBaseMod_concat, SeparatedBaseFile_concat; repeat rewrite map_app, in_app_iff, DeM1.
+        destruct HDisjRegs,(HDisjRegs0 k),(HDisjRegs1 k); dest;[left|right|left|right|left|left|right|right];split; auto.
+      * specialize (separateBaseModule_flatten_Rules (ConcatMod m1 m2)) as TMP1;
+        specialize (separateBaseModule_flatten_Rules m1) as TMP2; specialize (separateBaseModule_flatten_Rules m2) as TMP3.
+        unfold mergeSeparatedMod in *; rewrite getAllRules_createHide' in *; simpl in *; intro.
+        specialize (HDisjRules k); rewrite TMP2, TMP3 in HDisjRules.
+        repeat rewrite map_app,in_app_iff,DeM1 in *.
+        destruct (separateBaseMod m1), (separateBaseMod m2); simpl in *.
+        rewrite SeparatedBaseMod_concat_Rules, SeparatedBaseFile_concat_Rules; repeat rewrite map_app, in_app_iff, DeM1.
+        destruct HDisjRules,(HDisjRules0 k),(HDisjRules1 k); dest;[left|right|left|right|left|left|right|right];split; auto.
+      * specialize (separateBaseModule_flatten_Methods (ConcatMod m1 m2)) as TMP1;
+        specialize (separateBaseModule_flatten_Methods m1) as TMP2; specialize (separateBaseModule_flatten_Methods m2) as TMP3.
+        unfold mergeSeparatedMod in *; rewrite getAllMethods_createHide' in *; simpl in *; intro.
+        specialize (HDisjMeths k); rewrite TMP2, TMP3 in HDisjMeths.
+        repeat rewrite map_app,in_app_iff,DeM1 in *.
+        destruct (separateBaseMod m1), (separateBaseMod m2); simpl in *.
+        rewrite SeparatedBaseMod_concat_Meths, SeparatedBaseFile_concat_Meths; repeat rewrite map_app, in_app_iff, DeM1.
+        destruct HDisjMeths,(HDisjMeths0 k),(HDisjMeths1 k); dest;[left|right|left|right|left|left|right|right];split; auto.
+      * apply WfModBreakDownFile; econstructor; eauto.
+      * apply WfModBreakDownMod; econstructor; eauto.
+      * apply WfConcat_noHide.
+        apply mergeSeparatedBaseMod_noHides.
+      * apply WfConcat_noHide.
+        apply mergeSeparatedBaseFile_noHides.
+Qed.
+
+Definition WfMergedMod (m : WfModule) :  WfModule :=
+  (mkWfMod (merged_WellFormed (Wf_cond m))).
+
+Lemma merged_perm_equality m :
+  WfModule_perm m (WfMergedMod m).
+Proof.
+  constructor; simpl.
+  - apply separateBaseMod_flatten.
+  - apply separateBaseModule_flatten_Methods.
+  - apply separateBaseModule_flatten_Rules.
+  - apply separateBaseModule_flatten_Hides.
+Qed.
+
+Lemma TraceInclusion_Merge_l (m : WfModule) :
+  TraceInclusion m (WfMergedMod m).
+Proof.
+  apply PTraceInclusion_TraceInclusion.
+  - apply (Wf_cond m).
+  - apply (Wf_cond (WfMergedMod m)).
+  - repeat intro.
+    apply (PTrace_WfModule_rewrite (merged_perm_equality m)) in H.
+    exists ls.
+    split.
+    + unfold PTraceList; exists o; eauto.
+    + apply WeakInclusionsRefl.
+Qed.
+
+Lemma TraceInclusion_Merge_r (m : WfModule) :
+  TraceInclusion (WfMergedMod m) m.
+Proof.
+  apply PTraceInclusion_TraceInclusion.
+  - apply (Wf_cond (WfMergedMod m)).
+  - apply (Wf_cond m).
+  - repeat intro.
+    apply (PTrace_WfModule_rewrite (WfModule_perm_sym (merged_perm_equality m))) in H.
+    exists ls.
+    split.
+    + unfold PTraceList; exists o; eauto.
+    + apply WeakInclusionsRefl.
+Qed.
